SystemFD/Metatheory/Progress.lean
@@ -3,810 +3,656 @@ import SystemFD.Term
 import SystemFD.Ctx
 import SystemFD.Judgment
 import SystemFD.Metatheory.Classification
+import SystemFD.Metatheory.FrameWf
 import SystemFD.Metatheory.Inversion
 import SystemFD.Reduction
 
 inductive Val : Ctx Term -> Term -> Prop where
-  | app : t.neutral_form = .some (n, ts)
-        -> (Γ.is_stable_red n)
-        -> Val Γ t
-  | appk : Val Γ (f `@k a)
-  | lam :  Val Γ (`λ[a] b)
-  | lamt : Val Γ (Λ[A] b)
-  | refl : Val Γ (refl! _)
-  | star : Val Γ ★
-  | arr :  Val Γ (A -t> B)
-  | arrk : Val Γ (A -k> B)
-  | all : Val Γ (∀[A]B)
-  | eq : Val Γ (A ~ B)
+| app : t.neutral_form = .some (n, ts)
+      -> (Γ.is_stable_red n)
+      -> Val Γ t
+| lam :  Val Γ (`λ[a] b)
+| lamt : Val Γ (Λ[A] b)
+| refl : Val Γ (refl! _)
+| star : Val Γ ★
+| arr :  Val Γ (A -t> B)
+| arrk : Val Γ (A -k> B)
+| all : Val Γ (∀[A]B)
+| eq : Val Γ (A ~ B)
 
-
-theorem flip_eq : Γ ⊢ (A ~ B) : ★ -> Γ ⊢ (B ~ A) : ★ := by
-intros h; cases h; case _ k AJ BJ => apply Judgment.eq k BJ AJ
-
-theorem not_neutral_form_shape : Val Γ t ->
-        t.neutral_form = .some (n, ts)
-        -> ¬ ((t = `λ[A] b)
-            ∨ (t = Λ[A] b)
-            ∨ t = .letterm A t' b
-            ∨ t = .guard p s b
-            ∨ t = .ite p s b c
-            ∨ t = .kind
-            ∨ t = .type
-            -- ∨ t = refl! A
-            -- ∨ t = sym! η
-            ) := by
-intros tnf; induction t;
-any_goals (solve | simp_all)
-
-def DeclCtx (Γ : Ctx Term) : Prop := (∀ n,  ¬ Γ.is_type n)
-namespace DeclCtx
-theorem consempty : DeclCtx Γ -> DeclCtx (.empty :: Γ) := by
-  intros dctx; induction Γ;
+theorem val_sound_var_lemma :
+  t.neutral_form = .some (n, sp) ->
+  Γ.is_stable_red n ->
+  ∀ t', ¬ (Red Γ t t')
+:= by
+intro j1 j2 t' r
+induction t generalizing n sp Γ t'
+all_goals (try simp at j1)
+case _ x =>
+  cases j1; case _ e1 e2 =>
+    subst e1; subst e2
+    cases r
+    case _ x' sp' ix tl q1 q2 q3 q4 q5 =>
+      replace q1 := Frame.is_openm_destruct q1
+      cases q1; case _ q1 =>
+        simp at *; cases q4; case _ e1 e2 =>
+          subst e1; subst e2
+          unfold Frame.is_stable_red at j2
+          simp at j2; rw [q1] at j2; simp at j2
+    case _ s x' sp' t q1 q2 =>
+      simp at *; cases q2; case _ e1 e2 =>
+        subst e1; subst e2
+        rw [<-q1] at j2; unfold Frame.is_stable_red at j2
+        simp at j2
+case _ v t1 t2 ih1 ih2 =>
+  cases v; all_goals (try simp at j1)
   case _ =>
-    unfold DeclCtx; intro n xx; unfold Ctx.is_type at xx; unfold Frame.is_type at xx;
-    cases n;
-    case _ =>
-      simp_all; unfold Frame.apply at xx; simp at xx;
-    case _ => simp at xx; unfold Frame.apply at xx; simp at xx
-  case _ hf tl ih =>
-    unfold DeclCtx; unfold DeclCtx at dctx;
-    unfold Ctx.is_type;
-    sorry
-theorem conskind : DeclCtx Γ -> DeclCtx (.kind t :: Γ) := by sorry
+    rw [Option.bind_eq_some] at j1; simp at j1
+    cases j1; case _ a j1 =>
+    cases j1; case _ b j1 =>
+    cases j1; case _ h1 h2 =>
+    cases h2; case _ h2 h3 =>
+      subst h2; cases r <;> simp at *
+      case _ x sp' ix tl q1 q2 q3 q4 q5 =>
+        replace q4 := Eq.symm q4
+        rw [Option.bind_eq_some] at q4; simp at q4
+        cases q4; case _ u q4 =>
+        cases q4; case _ v q4 =>
+        cases q4; case _ w1 w2 =>
+        cases w2; case _ w2 w3 =>
+          subst w2; rw [w1] at h1
+          injection h1 with e
+          injection e with e1 e2
+          subst e1; subst e2
+          replace q1 := Frame.is_openm_destruct q1
+          cases q1; case _ q1 =>
+            rw [q1] at j2; unfold Frame.is_stable_red at j2
+            simp at j2
+      case _ s x sp' t q1 q2 =>
+        replace q2 := Eq.symm q2
+        rw [Option.bind_eq_some] at q2; simp at q2
+        cases q2; case _ u q2 =>
+        cases q2; case _ v q2 =>
+        cases q2; case _ w1 w2 =>
+        cases w2; case _ w2 w3 =>
+          subst w2; rw [w1] at h1
+          injection h1 with e
+          injection e with e1 e2
+          subst e1; subst e2
+          rw [<-q1] at j2; unfold Frame.is_stable_red at j2
+          simp at j2
+  case _ =>
+    rw [Option.bind_eq_some] at j1; simp at j1
+    cases j1; case _ a j1 =>
+    cases j1; case _ b j1 =>
+    cases j1; case _ h1 h2 =>
+    cases h2; case _ h2 h3 =>
+      subst h2; cases r <;> simp at *
+      case _ x sp' ix tl q1 q2 q3 q4 q5 =>
+        replace q4 := Eq.symm q4
+        rw [Option.bind_eq_some] at q4; simp at q4
+        cases q4; case _ u q4 =>
+        cases q4; case _ v q4 =>
+        cases q4; case _ w1 w2 =>
+        cases w2; case _ w2 w3 =>
+          subst w2; rw [w1] at h1
+          injection h1 with e
+          injection e with e1 e2
+          subst e1; subst e2
+          replace q1 := Frame.is_openm_destruct q1
+          cases q1; case _ q1 =>
+            rw [q1] at j2; unfold Frame.is_stable_red at j2
+            simp at j2
+      case _ s x sp' t q1 q2 =>
+        replace q2 := Eq.symm q2
+        rw [Option.bind_eq_some] at q2; simp at q2
+        cases q2; case _ u q2 =>
+        cases q2; case _ v q2 =>
+        cases q2; case _ w1 w2 =>
+        cases w2; case _ w2 w3 =>
+          subst w2; rw [w1] at h1
+          injection h1 with e
+          injection e with e1 e2
+          subst e1; subst e2
+          rw [<-q1] at j2; unfold Frame.is_stable_red at j2
+          simp at j2
+      case _ tl r e => apply ih1 h1 j2 tl r
+  case _ =>
+    rw [Option.bind_eq_some] at j1; simp at j1
+    cases j1; case _ a j1 =>
+    cases j1; case _ b j1 =>
+    cases j1; case _ h1 h2 =>
+    cases h2; case _ h2 h3 =>
+      subst h2; cases r <;> simp at *
+      case _ x sp' ix tl q1 q2 q3 q4 q5 =>
+        replace q4 := Eq.symm q4
+        rw [Option.bind_eq_some] at q4; simp at q4
+        cases q4; case _ u q4 =>
+        cases q4; case _ v q4 =>
+        cases q4; case _ w1 w2 =>
+        cases w2; case _ w2 w3 =>
+          subst w2; rw [w1] at h1
+          injection h1 with e
+          injection e with e1 e2
+          subst e1; subst e2
+          replace q1 := Frame.is_openm_destruct q1
+          cases q1; case _ q1 =>
+            rw [q1] at j2; unfold Frame.is_stable_red at j2
+            simp at j2
+      case _ s x sp' t q1 q2 =>
+        replace q2 := Eq.symm q2
+        rw [Option.bind_eq_some] at q2; simp at q2
+        cases q2; case _ u q2 =>
+        cases q2; case _ v q2 =>
+        cases q2; case _ w1 w2 =>
+        cases w2; case _ w2 w3 =>
+          subst w2; rw [w1] at h1
+          injection h1 with e
+          injection e with e1 e2
+          subst e1; subst e2
+          rw [<-q1] at j2; unfold Frame.is_stable_red at j2
+          simp at j2
+      case _ tl r e => apply ih1 h1 j2 tl r
 
-end DeclCtx
+theorem val_sound : Val Γ t -> ∀ t', ¬ (Red Γ t t') := by
+intro j; induction j
+case _ Γ t n sp j2 j3 =>
+  intro t' r
+  apply val_sound_var_lemma j2 j3 t' r
+all_goals (
+  case _ =>
+    intro t' r
+    cases r <;> simp at *
+)
 
-theorem no_lam_bindings : (DeclCtx Γ) -> (∀ x, ¬ (Γ d@ x = .type T)) := by
-intro dctx x h;
-have xx := @dctx x; simp at xx; rw[h] at xx; unfold Frame.is_type at xx; simp_all;
+theorem weaken_ctx_kind {Γ : Ctx Term}:
+  (∀ x, Ctx.is_type Γ x = false) ->
+  (∀ n, Ctx.is_type (.kind K :: Γ) n = false)
+:= by
+intro h n;
+cases n;
+case _ =>
+  simp; unfold Frame.apply; simp
+  unfold Frame.is_type; simp
+case _ n => simp at *; rw [<-Frame.is_type_apply]; apply h n
 
-theorem dt_is_dt {Γ : Ctx Term}: Γ d@x = Frame.datatype t -> (Γ d@ x).is_datatype := by
-intros dt; simp_all; unfold Frame.is_datatype; simp;
-
-theorem dt_is_stable {Γ : Ctx Term}{x : Nat}: Γ d@ x = Frame.datatype t -> Frame.is_stable_red (Γ d@ x) := by
-intros dt; unfold Frame.is_stable_red; rw [dt];
-
-theorem opent_is_stable {Γ : Ctx Term}: Γ d@x = Frame.opent t -> Frame.is_stable_red (Γ d@ x) := by
-intros dt; unfold Frame.is_stable_red; rw [dt];
-
-theorem apptneqrefl : ¬ ((f `@t a) = (refl! A)) := by simp_all
-theorem appneqrefl : ¬ ((f `@ a) = (refl! A)) := by simp_all
-
-theorem openm_no_stable {Γ : Ctx Term}{n : Nat} :
-  Frame.is_openm (Γ d@ n) = true -> ¬ (Frame.is_stable_red (Γ d@ n)) := by
-intros om; simp_all; unfold Frame.is_openm at om; split at om;
-case _ => unfold Frame.is_stable_red; simp_all;
-case _ => simp_all
-
-theorem stable_no_reduce : t.neutral_form = .some (n, sp) -> Γ.is_stable_red n = true -> ¬ ∃ t', Red Γ t t' := by
-intros tnf nstable x; cases x;
-  case _ w h =>
-  simp_all; induction h generalizing n sp;
-  any_goals (solve | simp_all)
-  case _ Γ _ _ _ _ om _ _ nstable =>
-    have n_not_stable := openm_no_stable om;
-    simp_all;
-  case _ hnf idx =>
-    unfold Frame.is_stable_red at nstable; symm at hnf;
-    have uniq' := Term.unique_neutral_form hnf tnf; have uniq := uniq'.1;
-    subst uniq; rw [<-idx] at nstable; simp_all
-  case _ f _ _ a _ _ ih =>
-    simp_all; rw[Option.bind_eq_some] at tnf;
-    cases tnf; case _ w h =>
-      have fa_spine := @Term.neutral_form_app f a w.fst w.snd h.1;
-      have f_spine := Term.neutral_form_app_rev fa_spine;
-      have xx := @ih w.1 w.2 f_spine; simp at h;
-      have wfst := And.left (And.right h); symm at wfst;
-      subst wfst; simp_all;
-  case _ ih =>
-    simp_all; rw [Option.bind_eq_some] at tnf;
-    cases tnf; case _ f _ _ a _ _ w h =>
-      have fa_spine := @Term.neutral_form_appt f a w.fst w.snd h.1;
-      have f_spine := Term.neutral_form_appt_rev fa_spine;
-      have xx := @ih w.1 w.2 f_spine; simp at h;
-      have wfst := And.left (And.right h); symm at wfst;
-      subst wfst; simp_all;
+theorem weaken_ctx_empty {Γ : Ctx Term}:
+  (∀ x, Ctx.is_type Γ x = false) ->
+  (∀ n, Ctx.is_type (.empty :: Γ) n = false)
+:= by
+intro h n;
+cases n;
+case _ =>
+  simp; unfold Frame.apply; simp
+  unfold Frame.is_type; simp
+case _ n => simp at *; rw [<-Frame.is_type_apply]; apply h n
 
 @[simp]
-abbrev ValueNoSteps : (v : JudgmentVariant) -> (Γ : Ctx Term)  -> (JudgmentArgs v) -> Prop
-| .prf => λ Γ => λ(t , _) => Val Γ t -> ¬ ∃ t', Red Γ t t'
+abbrev TypesAreValuesLemmaType : (v : JudgmentVariant) -> (Γ : Ctx Term) -> (JudgmentArgs v) -> Prop
+| .prf => λ Γ => λ(t , K) => Γ ⊢ K : .kind -> Val Γ t
 | .wf  => λ _ => λ () => true
 
-
-theorem val_no_red :
-  DeclCtx Γ ->
+theorem types_are_values_lemma :
   Judgment v Γ ix ->
-  ValueNoSteps v Γ ix
-  := by
-intros dctx tJ; have wΓ := judgment_ctx_wf tJ;
-induction tJ;
-any_goals(solve | simp_all)
-all_goals(intro vt treds; cases treds; cases vt; simp_all)
-case _ h =>
-  cases h;
-  case _ => simp_all
-  case _ => simp_all
-case _ h _ _ =>
-  cases h;
-  case _  n _ x_stable _ _ _ _ _ x_openm _ _ nnf _ =>
-    symm at nnf; have nnf' := @Term.var_neutral_form n; rw[nnf'] at nnf; injection nnf with nnf; simp at nnf;
-    have x_n := nnf.1; rw[<-x_n] at x_openm;
-    have x_not_stable := Frame.is_openm_implies_not_is_stable_red x_openm; contradiction;
-  case _ n' _ x_stable _ _ n _ _ x_term nnf =>
-    symm at nnf; have nnf' := @Term.var_neutral_form n'; rw[nnf'] at nnf; simp at nnf;
-    have n_n := nnf.1; rw[n_n] at x_stable; rw[<-x_term] at x_stable;
-    unfold Frame.is_stable_red at x_stable; simp at x_stable;
-case _ h =>
-  cases h;
-  case _ h _ => cases h
-  case _ h => cases h
-case _ h =>
-  cases h;
-  case _ h _ => cases h
-  case _ h => cases h
-case _ h =>
-  cases h
-  case _ h _ => cases h
-  case _ h => cases h
-case _ h =>
-  rw [Option.bind_eq_some] at h; cases h
-  case _ h _ _ _ =>
-    cases h;
-    case _ _ x_stable _ _ _ _ _ _ x_openm _ _ hh _ =>
-      simp_all; have hh := hh.1; subst hh; simp_all;
-      have x_not_stable := Frame.is_openm_implies_not_is_stable_red x_openm; contradiction;
-    case _ Γ f _ _ arg _ _ n ts _ _ x_stable w fnfp _ x sp _ x_term hh =>
-      have fnf := fnfp.2;
-      injection fnf with fnf;
-      have weqx : w.fst = n := by simp_all;
-      have tseqw :  w.snd ++ [(.kind, arg)]= ts := by simp_all;
-      symm at tseqw;
-      symm at hh;
-      subst weqx; subst tseqw;
-      have xx := Term.neutral_form_appk_rev_exists hh; cases xx;
-      case _ fnfp =>
-        have hh := fnfp.2; subst hh; simp_all;
-        have hh1 := hh.1; have hh2 := hh.2;
-        have xterm : Γ.is_term x = true := by simp; unfold Frame.is_term; rw[<-x_term];
-        have x_not_stable := Frame.is_term_implies_not_is_stable_red xterm; apply (x_not_stable x_stable);
-case _ Γ f _ _ a fj _ _ _ _ h =>
-  cases h;
-  case _ =>
-    have lem := classification_lemma fj; simp at lem;
-    cases lem;
-    case _ => simp_all; sorry
-    case _ h => cases h; case _ w h => sorry
+  TypesAreValuesLemmaType v Γ ix
+:= by
+intro j; induction j <;> simp at *
+all_goals (intro h1)
+case _ j _ _ _ _ =>
+  have lem := uniqueness_of_types j h1
+  injection lem
+case _ => cases h1
+case _ Γ x T j1 j2 _ =>
+  generalize fdef : Γ d@ x = f at *
+  have lem := frame_wf_by_index x j1
+  rw [fdef] at lem
+  cases lem
+  all_goals (
+    unfold Frame.get_type at j2
+    simp at j2
+  )
+  case type j3 =>
+    subst j2
+    have lem := uniqueness_of_types h1 j3
+    injection lem
+  case openm j3 =>
+    subst j2
+    have lem := uniqueness_of_types h1 j3
+    injection lem
+  case term j3 _ =>
+    subst j2
+    have lem := uniqueness_of_types h1 j3
+    injection lem
+  all_goals (
+    case _ =>
+      subst j2; apply @Val.app Γ #x x []
+      simp; simp; rw [fdef]; unfold Frame.is_stable_red
+      simp
+  )
+case _ => cases h1
+case _ => apply Val.all
+case _ => apply Val.arr
+case _ Γ f A B a j1 j2 ih1 ih2 =>
+  have lem := classification_lemma j1 <;> simp at lem
+  cases lem
+  case _ lem =>
+    replace ih1 := ih1 lem
+    cases ih1
+    case app x sp q1 q2 =>
+      apply @Val.app Γ (f `@k a) x (sp ++ [(.kind, a)])
+      simp; rw [Option.bind_eq_some]; simp; apply q2
+      apply q1
+    all_goals (cases j1)
+  case _ lem =>
+    cases lem; case _ K lem =>
+      cases lem.2; cases lem.1
+case _ => apply Val.eq
+case _ j _ _ _ _ _ _ _ =>
+  have lem := uniqueness_of_types j h1
+  injection lem
+case _ j _ _ _ _ _ =>
+  have lem := uniqueness_of_types j h1
+  injection lem
+case _ => apply Val.lam
+case _ Γ f A B a B' j1 j2 j3 ih1 ih2 =>
+  have lem := classification_lemma j1
+  cases lem <;> simp at *
+  case _ lem =>
+    cases lem <;> simp at *
+    case _ lem => cases lem
+    case _ lem =>
+      cases lem; case _ K lem =>
+      cases lem.2; case _ j4 j5 =>
+        replace j5 := beta_empty a j5; simp at j5
+        rw [j3] at h1
+        have lem := uniqueness_of_types h1 j5
+        injection lem
+case _ => apply Val.lamt
+case _ Γ f A B a B' j1 j2 j3 ih1 ih2 =>
+  have lem := classification_lemma j1
+  cases lem <;> simp at *
+  case _ lem =>
+    cases lem <;> simp at *
+    case _ lem => cases lem
+    case _ lem =>
+      cases lem; case _ K lem =>
+      cases lem.2; case _ j4 j5 =>
+        replace j5 := beta_kind j5 j2; simp at j5
+        rw [j3] at h1
+        have lem := uniqueness_of_types h1 j5
+        injection lem
+case _ j _ _ =>
+  have lem := classification_lemma j <;> simp at lem
+  cases lem
+  case _ lem => cases lem
+  case _ lem =>
+    cases lem; case _ K lem =>
+    cases lem.2; case _ q _ j2 =>
+      have lem2 := uniqueness_of_types h1 j2
+      subst lem2; cases q
+case _ => apply Val.refl
+all_goals (case _ => cases h1)
 
-  case _ T x sp t x_term fanf =>
-    symm at fanf; have fanf := Term.neutral_form_appk_rev_exists fanf;
-    cases fanf; case _ fsp fanf =>
-    symm at x_term; symm at fanf;
-    have xx := ctx_get_term_well_typed wΓ x_term;
-    sorry
-    -- have xx' := ctx_get_term_type_kind wΓ x_term;
-    -- have lem := classification_lemma xx.1; simp at lem; cases lem;
-    -- case _ h => subst h; cases xx'.2;
-    -- case _ h =>
-    --   cases h;
-    --   case _ h => have uniq := uniqueness_of_types xx'.2 h; simp_all;
-    --   case _ h => sorry
-          -- cases h; case _ h =>
-          --   have uniq := uniqueness_of_types xx' h.2; subst uniq;
-          --   have f_form := Term.neutral_form_law fp; subst f_form; simp_all;
-          --   case _ fj => sorry
-case _ h =>
-  cases h;
-  case _ => simp_all
-  case _ => simp_all
-case _ h =>
-  cases h;
-  case _ => simp_all
-  case _ => simp_all
-case _ h' _ h =>
-  rw[Option.bind_eq_some] at h;
-  cases h'
-  case _ => simp_all;
-  case _ => sorry
-  case _ => sorry
-  case _ => sorry
-case _ h =>
-  cases h;
-  case _ => simp_all
-  case _ => simp_all
-case _ h' _ h =>
-  rw[Option.bind_eq_some] at h;
-  cases h; case _ fnf =>
-    cases h';
-    case _ => simp_all
-    case _ => simp_all; sorry
-    case _ => sorry
-    case _ => sorry
-case _ h =>
-  cases h;
-  case _ => simp_all
-  case _ => simp_all
+theorem types_are_values :
+  Γ ⊢ t : K ->
+  Γ ⊢ K : .kind ->
+  Val Γ t
+:= by
+intro j1 j2
+apply types_are_values_lemma j1 j2
 
--- s is a value, cannot have a neutral form; datatype type, is impossible
-theorem term_neutral_form_datatype :
-  Val Γ t ->
-  t.neutral_form = .none ->
-  ValidHeadVariable T Γ.is_datatype ->
-  Γ ⊢ t : T ->
-  False := by
-intros tv nf vhv tJ;
-induction tv;
-any_goals (solve | simp_all)
-any_goals (solve | cases tJ; cases vhv; simp_all)
-case _ Γ f h =>
-  have lem := type_disjoint tJ; simp at lem;
-  unfold ValidHeadVariable at vhv;
-  sorry
-
-theorem term_neutral_form_opent :
-  Val Γ t ->
-  t.neutral_form = .none ->
-  ValidHeadVariable T Γ.is_opent ->
-  Γ ⊢ t : T ->
-  False := by
-intros tv nf vhv tJ;
-sorry
-
-
-theorem var_type_lemma :
+theorem refl_var_spine_lemma :
   Γ.is_stable_red n ->
-  Γ ⊢ (#n).apply_spine ts : (A ~ B)
-  -> False := by
-intros n_stable h; induction ts;
-case _ => simp_all; cases h; case _ wΓ ty => symm at ty;  apply (ctx_get_var_no_eq_type wΓ n_stable ty);
-case _ hd tl ih =>
-   sorry
+  Γ ⊢ (#n).apply_spine sp : (A ~ B) ->
+  False
+:= by
+intro j1 j2
+have lem := inversion_apply_spine j2
+cases lem; case _ C lem =>
+cases lem; case _ h1 h2 =>
+cases h2; case _ j3 j4 =>
+  have lem := classification_lemma j2 <;> simp at lem
+  cases lem
+  case _ lem => cases lem
+  case _ lem =>
+    cases lem; case _ K lem =>
+    cases lem.2; case _ q1 q2 q3 =>
+      apply ctx_get_var_no_spine_eq_type j3 j1
+      rw [j4]; apply lem.2; apply h1
 
-
-theorem var_well_typed :
-  Γ.is_stable_red n ->
-  Γ ⊢ #n : (A ~ B)
-  -> False := by
-intros n_stable tJ; cases tJ;
-case _ wΓ ty =>
-  symm at ty; apply (ctx_get_var_no_eq_type wΓ n_stable ty);
-
-theorem var_app_well_typed :
-  Γ.is_stable_red n ->
-  Γ ⊢ (#n `@ t) : (A ~ B)
-  -> False := by
-intros n_stable tJ;
-cases tJ;
-case _ nJ tJ eq =>
-  cases nJ;
-  case _ wΓ nty =>
-    symm at nty; induction Γ;
-    case _ => unfold Frame.get_type at nty; simp at nty
-    case _ hf tlf ih =>
-         unfold Ctx.is_stable_red at n_stable; unfold Frame.is_stable_red at n_stable; simp at n_stable;
-         sorry
-
-theorem refl_is_val : DeclCtx Γ -> Γ ⊢ η : (A ~ B)
-                    -> Val Γ η
-                    -> η = refl! A ∧ A = B := by
-intros dctx ηJ vη; induction vη;
+theorem refl_is_val :
+  Γ ⊢ η : (A ~ B) ->
+  Val Γ η ->
+  η = refl! A ∧ A = B
+:= by
+intros ηJ vη; induction vη;
 any_goals(solve | cases ηJ)
 case _ Γ t n ts tnf n_stable =>
      symm at tnf; replace tnf := Term.neutral_form_law tnf;
-     subst tnf; exfalso; apply (var_type_lemma n_stable ηJ);
+     subst tnf;
+     exfalso;
+     apply (refl_var_spine_lemma n_stable ηJ);
 case _ => cases ηJ; case _ fJ =>
   have lem := classification_lemma fJ; simp at lem; cases lem;
-  case _ h => cases h; case _ h => have h := invert_eq_kind h; cases h;
-  case _ h => cases h; case _ h => simp_all; cases h.2; cases h.1
-case _ => cases ηJ; simp_all
-
-theorem ctor_uniqueness {Γ : Ctx Term}: (Γ.is_ctor x = true) -> (Γ.is_ctor y = false) -> x ≠ y := by
-intros xctor yctor xeqy ;
-induction Γ;
-case _ => simp_all
-case _ here there ih =>
-  unfold Ctx.is_ctor at xctor; unfold dnth at xctor;
-  split at xctor;
-  case _ => simp_all;
-  case _ =>
-    simp_all; subst xeqy;
-    unfold dnth at yctor; simp_all;
-  case _ =>
-    simp_all; subst xeqy;
-    unfold dnth at yctor; simp_all;
-
-theorem insttype_uniqueness {Γ : Ctx Term}: (Γ.is_insttype x = true) -> (Γ.is_insttype y = false) -> x ≠ y := by
-intros xinst yinst xeqy ;
-induction Γ;
-case _ => simp_all
-case _ here there ih =>
-  unfold Ctx.is_insttype at xinst; unfold dnth at xinst;
-  split at xinst;
-  case _ => simp_all;
-  case _ =>
-    simp_all; subst xeqy;
-    unfold dnth at yinst; simp_all;
-  case _ =>
-    simp_all; subst xeqy;
-    unfold dnth at yinst; simp_all;
-
-
--- this is stupid
-theorem bool_implication (x : Bool) : x = false -> ¬ x = true :=
-by intro h; rw [h]; simp
-
-
-theorem head_cannot_be_empty :
-   DeclCtx Γ ->
-   Γ ⊢ t : T ->
-   .some (x, sp) = Term.neutral_form t ->
-   ¬ Γ d@ x  = .empty
-:= by
-intros dctx tJ tnf x_empty;
-induction sp
-case _ =>
-  simp_all;
-  have xx' := Term.neutral_form_law tnf; unfold Term.apply_spine at xx';
-  rw [<-xx'] at tJ;
-  cases tJ; case _ h => rw [x_empty] at h; unfold Frame.get_type at h; simp at h
-case _ ht tl ih =>
-  have xx := Term.neutral_form_law tnf;
-
-  sorry
-
-
-theorem unstable_var_steps :
-   (∀ n,  ¬ Γ.is_type n) ->
-   Γ ⊢ t : T ->
-   .some (x, sp) = Term.neutral_form t ->
-   (Γ.is_stable_red x = false) ->
-   ∃ t', Red Γ t t'
-:= by
-intros dctx tJ tnf x_not_stable;
-have x_not_stable := @bool_implication (Γ.is_stable_red x) x_not_stable;
-generalize xx : Γ d@ x = f;
-cases f;
-any_goals (solve | unfold Ctx.is_stable_red at x_not_stable
-                   rw [xx] at x_not_stable
-                   simp at x_not_stable
-                   unfold Frame.is_stable_red at x_not_stable
-                   simp at x_not_stable)
-case empty =>
-  have no_empty := (head_cannot_be_empty dctx tJ tnf);
-  exfalso; apply (no_empty xx)
-case type => have xx' := @dctx x; unfold Ctx.is_type at xx'; rw [xx] at xx'; unfold Frame.is_type at xx'; simp_all;
-case term lt =>
-  symm at xx; have reds := Red.letterm tnf xx;
-  apply Exists.intro [lt.apply_spine sp] reds;
-case openm =>
-   have om : (Γ d@ x).is_openm := by unfold Frame.is_openm; rw [xx];
-   generalize isp : instance_indices Γ 0 x [] = ιs at *; symm at isp;
-   generalize instsp : get_instances Γ ιs = insts at *; symm at instsp;
-   generalize instsp' : List.map (·.apply_spine sp) insts = insts' at *; symm at instsp';
-   apply (Exists.intro insts' (Red.inst tnf om isp instsp instsp'))
+  case _ h => cases h; case _ h => cases h
+  case _ h => apply And.intro rfl rfl
 
 @[simp]
-abbrev StepOrVal : (v : JudgmentVariant) -> (Γ : Ctx Term) -> (JudgmentArgs v) -> Prop
+abbrev ProgressLemmaType : (v : JudgmentVariant) -> (Γ : Ctx Term) -> (JudgmentArgs v) -> Prop
 | .prf => λ Γ => λ(t , _) => Val Γ t ∨ ∃ t', Red Γ t t'
 | .wf  => λ _ => λ () => true
 
-theorem progress :
-   ⊢ Γ -> (∀ n,  ¬ Γ.is_type n)
-  -> Judgment v Γ ix
---------------------------------------
-  -> StepOrVal v Γ ix := by
-intros wΓ ntype j; induction j;
-any_goals (solve | simp_all)
-case _ Γ A t b _ _ _ _ _ _ _ ih _ =>
-  simp_all;
-  generalize tl' : [b β[ t ]] = t' at *; symm at tl';
-  have reds := @Red.letbeta Γ A t b; rw [<-tl']  at reds;
-  have ereds : ∃ t', Red Γ (.letterm A t b) t' := Exists.intro t' reds;
-  apply Or.inr ereds;
-
-case _ => simp_all; apply Or.inl Val.star;
-case var Γ x _ _ xTy ih =>
-  simp at ih;
-  unfold Frame.get_type at xTy; simp at xTy;
-  split at xTy;
-  any_goals (solve | simp_all)
-  case _ f _ x_is_kind => -- bogus case
-    simp_all; have xK := ctx_get_var_type wΓ x_is_kind;
-    have hh : (#x).neutral_form = .some (x, []) := Term.var_neutral_form;
-    have k_st_red : Γ.is_stable_red x := by simp; unfold Frame.is_stable_red; rw [x_is_kind]
-    apply Or.inl (Val.app hh k_st_red);
-  case _ f _ x_is_type =>
-    exfalso; have ntype' := ntype x; simp at ntype'; rw[x_is_type] at ntype';
-    unfold Frame.is_type at ntype'; simp at ntype';
-  case _ f _ x_is_datatype =>
-      simp_all; have x_is_stable := dt_is_stable x_is_datatype;
-      have hh : (#x).neutral_form = .some (x, []) := Term.var_neutral_form;
-      apply Or.inl;
-      apply Val.app hh x_is_stable;
-  case _ f t x_is_ctor =>
-    have xx : Frame.is_stable_red (Γ d@ x) := by unfold Frame.is_stable_red; rw[x_is_ctor];
-    have hh : (#x).neutral_form = .some (x, []) := Term.var_neutral_form;
-    apply Or.inl (Val.app hh xx)
-  case _ x_is_opent =>
-      have x_is_stable := opent_is_stable x_is_opent;
-      have hh : (#x).neutral_form = .some (x, []) := Term.var_neutral_form;
-      apply Or.inl;
-      apply Val.app hh x_is_stable;
-  case _ x_is_openm =>  -- steps inst
-    have nf  := @Term.var_neutral_form x; symm at nf;
-    have om : (Γ d@ x).is_openm := by unfold Frame.is_openm; rw [x_is_openm];
-    generalize isp : instance_indices Γ 0 x [] = ιs at *; symm at isp;
-    generalize instsp : get_instances Γ ιs = insts at *; symm at instsp;
-    generalize instsp' : List.map (·.apply_spine []) insts = insts' at *; symm at instsp';
-    apply Or.inr (Exists.intro insts' (Red.inst nf om isp instsp instsp'))
-  case _ x_is_insttype =>  -- value
-    have xx : Frame.is_stable_red (Γ d@ x) := by unfold Frame.is_stable_red; rw[x_is_insttype];
-    have hh : (#x).neutral_form = .some (x, []) := Term.var_neutral_form;
-    apply Or.inl (Val.app hh xx)
-  case _ A t x_frame =>  -- steps letterm
-    have nf : .some (x, []) = (#x).neutral_form := Term.var_neutral_form;
-    have x_is_term : .term A t = Γ d@ x := by symm at x_frame; apply x_frame
-    generalize tlp : [t.apply_spine []] = t' at *; symm at tlp;
-    have etl' : ∃ t', Red Γ (#x) t' := Exists.intro ([t.apply_spine []]) (Red.letterm nf x_is_term);
-    apply Or.inr etl'
-
-case _ => simp_all; apply Or.inl; apply Val.arrk
-case _ => simp_all; apply Or.inl; apply Val.all
-case _ => simp_all; apply Or.inl; apply Val.arr
-
-case appk fs as => simp_all;  apply Or.inl; apply Val.appk
-
-case _ => simp_all; apply Or.inl; apply Val.eq
-
-case ite Γ p A s _ i _ _ e _ sJ RJ _ vhvp vhvr stm _ tstar _ ps ss _ is _ es =>
-  cases vhvp; case _ pf h =>
-    have pnf := h.1; have hpctor := h.2;
-    have p_n := pf.1; have p_sp := pf.2;
-    generalize snf : s.neutral_form = xx at *; symm at snf;
-    cases xx;
-    case _ =>
-       cases (ss wΓ ntype)
-       case _ h => exfalso; symm at snf; apply (term_neutral_form_datatype h snf vhvr sJ)
-       case _ h => cases h; case _ w h =>
-          generalize tlp : List.map (Term.ite p · i e) w = tl' at *; symm at tlp;
-          have reds : ∃ t', Red Γ (.ite p s i e) t' := Exists.intro tl' (Red.ite_congr h tlp);
-          apply Or.inr reds
-    case _ sf =>
-       simp;
-       have s_sp := sf.2;
-       generalize sp : sf.1 = s_n at *; symm at sp;
-       generalize s_spp : sf.2 = s_sp at *; symm at s_spp;
-       generalize snctor : Γ.is_ctor s_n = p at *;
-       have s_form := Term.neutral_form_law snf; rw[<-s_spp] at s_form; rw[<-sp] at s_form;
-       cases p;
-       case _ => -- scrutinee is a not ctor headed but has a neutral form
-         generalize xx : Γ.is_stable_red s_n = x_is_stable;
-         cases x_is_stable;
-         case false =>
-           apply Or.inr; simp at xx; rw[sp] at xx;
-           have reds' := unstable_var_steps ntype sJ snf xx;
-           cases reds'; case _ w sreds =>
-           generalize tlp : List.map (Term.ite p · i e) w = tl at *; symm at tlp;
-           have reds : ∃ t', Red Γ (.ite p s i e) t' := Exists.intro tl (Red.ite_congr sreds tlp)
-           apply reds
-         case true =>
-           generalize xx' : Γ d@ s_n = f;
-           cases f;
-           any_goals (solve | unfold Ctx.is_stable_red at xx; rw [xx'] at xx; unfold Frame.is_stable_red at xx; simp at xx)
-           any_goals (solve | subst sp;
-                              have reds : ∃ t', Red Γ (.ite p s i e) t' :=
-                                Exists.intro [e] (Red.ite_missed pnf snf xx (Or.inl (ctor_uniqueness hpctor snctor)));
-                              apply Or.inr; apply reds)
-
-       case _ =>
-          have check := Nat.decEq pf.fst sf.fst;
-          cases check;
-          case _ h =>
-            have s_is_stable : Γ.is_stable_red sf.fst := by rw[sp] at snctor; apply Frame.is_ctor_implies_is_stable_red snctor;
-            have reds : ∃ t', Red Γ (.ite p s i e) t' := Exists.intro [e] (Red.ite_missed pnf snf s_is_stable (Or.inl h));
-            apply Or.inr; apply reds;
-          case _ h =>
-            generalize comp_prefix : prefix_equal pf.snd sf.snd = h at *;
-            cases h
-            case _ h =>
-              have s_is_stable : Γ.is_stable_red sf.fst := by rw[sp] at snctor; apply Frame.is_ctor_implies_is_stable_red snctor;
-              have reds : ∃ t', Red Γ (.ite p s i e) t' :=
-                   Exists.intro [e] (Red.ite_missed pnf snf s_is_stable (Or.inr comp_prefix));
-              apply Or.inr; apply reds;
-            case _ h' =>
-              symm at comp_prefix;
-              have sfp : sf = (sf.fst , sf.snd) := by simp_all;
-              rw [sfp] at snf; rw[<-h] at snf;
-              have reds : ∃ t', Red Γ (.ite p s i e) t' :=
-                Exists.intro [i.apply_spine h'] (Red.ite_matched pnf snf comp_prefix hpctor);
-              apply Or.inr; apply reds;
-
-case guard Γ p A s R t _ _ pJ sJ _ _ vhvp vhvr _ _ _  ps ss _ _ _  =>
-  cases vhvp; case _ pf h =>
-    have pnf := h.1; have hpctor := h.2;
-    have p_n := pf.1; have p_sp := pf.2;
-    generalize snf : s.neutral_form = xx at *; symm at snf;
-    cases xx;
-    case _ =>
-       cases (ss wΓ ntype)
-       case _ h => exfalso; symm at snf; apply (term_neutral_form_opent h snf vhvr sJ)
-       case _ h => cases h; case _ w h =>
-          generalize tlp : List.map (Term.guard p · t) w = tl' at *; symm at tlp;
-          have reds : ∃ t', Red Γ (.guard p s t) t' := Exists.intro tl' (Red.guard_congr h tlp);
-          apply Or.inr reds
-    case _ sf =>
-       simp
-       generalize snctor : Γ.is_insttype sf.fst = p at *;
-       generalize sp : sf.1 = s_n at *; symm at sp;
-       generalize s_spp : sf.2 = s_sp at *; symm at s_spp;
-       have s_form := Term.neutral_form_law snf; rw[<-s_spp] at s_form; rw[<-sp] at s_form;
-       cases p;
-       case _ =>   -- scrutinee is a not a opentype headed but has a neutral form
-         generalize xx : Γ.is_stable_red s_n = x_is_stable;
-         cases x_is_stable;
-         case false =>
-           apply Or.inr; simp at xx; rw[sp] at xx;
-           have reds' := unstable_var_steps ntype sJ snf xx;
-           cases reds'; case _ w sreds =>
-           generalize tlp : List.map (Term.guard p · t) w = tl at *; symm at tlp;
-           have reds : ∃ t', Red Γ (Term.guard p s t) t' := Exists.intro tl (Red.guard_congr sreds tlp)
-           apply reds
-         case true =>
-           generalize xx' : Γ d@ s_n = f;
-           cases f;
-           any_goals (solve | unfold Ctx.is_stable_red at xx; rw [xx'] at xx; unfold Frame.is_stable_red at xx; simp at xx)
-           any_goals (solve | subst sp;
-                              have reds : ∃ t', Red Γ (.guard p s t) t' :=
-                                Exists.intro [] (Red.guard_missed pnf snf xx (Or.inl (insttype_uniqueness hpctor snctor)));
-                              apply Or.inr; apply reds)
-       case _ =>
-          have check := Nat.decEq pf.fst sf.fst;
-          cases check;
-          case _ h =>
-            have s_is_stable : Γ.is_stable_red sf.fst := by rw[sp] at snctor; apply Frame.is_insttype_implies_is_stable_red snctor;
-            have reds : ∃ t', Red Γ (.guard p s t) t' := Exists.intro [] (Red.guard_missed pnf snf s_is_stable (Or.inl h));
-            apply Or.inr; apply reds; -- sorry
-          case _ h =>
-            generalize comp_prefix : prefix_equal pf.snd sf.snd = h at *;
-            cases h
-            case _ h =>
-              have s_is_stable : Γ.is_stable_red sf.fst := by rw[sp] at snctor; apply Frame.is_insttype_implies_is_stable_red snctor;
-              have reds : ∃ t', Red Γ (.guard p s t) t' :=
-                   Exists.intro [] (Red.guard_missed pnf snf s_is_stable (Or.inr comp_prefix));
-              apply Or.inr; apply reds;
-            case _ h' =>
-              symm at comp_prefix;
-              have sfp : sf = (sf.fst , sf.snd) := by simp_all;
-              rw [sfp] at snf; rw[<-h] at snf;
-              have reds : ∃ t', Red Γ (.guard p s t) t' :=
-                Exists.intro [t.apply_spine h'] (Red.guard_matched pnf snf comp_prefix);
-              apply Or.inr; apply reds;
-
-case _ _ A t _ _ _ _ _ _ _ => apply Or.inl Val.lam
-
-case app Γ f A B a B' fJ aJ _ fs as =>
-  have fs' := fs wΓ ntype;
-  cases fs'
-  case inl h => -- f is value
-    cases h;
-    case app n ts n_stable fnf =>
-       have fanf := @Term.neutral_form_app f a n ts fnf;
-       apply Or.inl (Val.app fanf n_stable);
-    case lam A B =>
-      apply Or.inr;
-      have reds : ∃ t', Red Γ ((`λ[A]B) `@ a) t' := Exists.intro [B β[ a ]] (@Red.beta Γ A B a);
-      apply reds
-    case lamt  => have xx := lamt_typing_unique fJ; cases xx; case _ w h => cases h;
-    case refl => have xx := refl_typing_unique fJ; cases xx
-    case _ => cases fJ; case _ fJ' =>
-      have lem := classification_lemma fJ'; simp at lem; cases lem;
-      case _ h => cases h; case _ h => cases h;
-      case _ h => cases h; case _ h => cases h.2; cases h.1;
-    case _ => have fJ' := Judgment.ax wΓ; have u := uniqueness_of_types fJ fJ'; cases u;
-    case _ => cases fJ
-    case _ => cases fJ;
-    case _ => cases fJ
-    case _ => cases fJ
-
-  case inr h => cases h; case _ w h => -- f steps
-    generalize tlp : List.map (· `@ a) w = tl' at *; symm at tlp;
-    have reds : ∃ t', Red Γ (f `@ a) t' := Exists.intro tl' (Red.app_congr h tlp);
-    apply Or.inr reds
-
-case _ _ A t _ _ _ _ _ _ _ => apply Or.inl Val.lamt
-
-case appt Γ f _ _ a _ fJ aJ _ fs as =>
-  cases fs wΓ ntype;
-  case inr h => cases h; case _ w h =>
-      apply Or.inr;
-      generalize tlp : List.map (· `@t a) w = tl' at *; symm at tlp;
-      have reds : ∃ t', Red Γ (f `@t a) t' := Exists.intro tl' (Red.appt_congr h tlp);
-      apply reds;
-  case inl h =>
-    cases h;
-    case app n ts n_stable fnf =>
-      have fanf := @Term.neutral_form_appt f a n ts fnf
-      apply Or.inl;
-      apply (Val.app fanf n_stable);
-    case lam => have xx := lam_typing_unique fJ; cases xx; simp_all;
-    case lamt a' b =>
-      apply Or.inr;
-      have reds : ∃ t', Red Γ ((Λ[a']b) `@t a) t' := Exists.intro [b β[ a ]] (@Red.betat Γ a' b a);
-      apply reds
-    case refl => have xx := refl_typing_unique fJ; cases xx
-    case _ => cases fJ; case _ fJ' =>
-      have lem := classification_lemma fJ'; simp at lem; cases lem;
-      case _ h => cases h; case _ h => cases h;
-      case _ h => cases h; case _ h => cases h.2; cases h.1;
-    case _ => have fJ' := Judgment.ax wΓ; have xx := uniqueness_of_types fJ fJ'; cases xx
-    case _ => cases fJ
-    case _ => cases fJ
-    case _ => cases fJ
-    case _ => cases fJ
-
-case _ Γ t A η B tJ ηJ ts cs =>
-  cases (cs wΓ ntype);
-  case _ h =>
-      have ηreflp := @refl_is_val Γ η A B ntype ηJ h;
-      have ηrefl := ηreflp.1;
-      subst ηrefl; apply Or.inr;
-      have reds : ∃ t', Red Γ (t ▹ refl! A) t' := Exists.intro [t] Red.cast;
-      apply reds
-  case _ h => cases h; case _ w h =>
-      apply Or.inr
-      generalize tlp : List.map (t ▹ ·) w = tl' at *; symm at tlp;
-      have reds : ∃ t', Red Γ (t ▹ η) t' := Exists.intro tl' (Red.cast_congr h tlp);
-      apply reds;
-
-case _ => apply Or.inl Val.refl
-case sym Γ η A B ηJ ηs =>
-  cases ηs wΓ ntype;
-  case _ h =>
-    have x := refl_is_val ntype ηJ h;
-    have xeqrefl := x.left;
-    have aeqB := x.right;
-    subst xeqrefl;
+theorem progress_lemma :
+  (∀ x, ¬ Γ.is_type x) ->
+  Judgment v Γ ix ->
+  ProgressLemmaType v Γ ix
+:= by
+intro h1 j
+induction j <;> try simp at *
+case _ =>
+  apply Or.inr; apply Exists.intro _
+  apply Red.letbeta
+case _ => apply Or.inl; apply Val.star
+case _ Γ x T j1 j2 _ =>
+  generalize fdef : Γ d@ x = f at *
+  cases f
+  case term A t =>
+    apply Or.inr; apply Exists.intro _
+    apply @Red.letterm A #x x [] Γ t
+    simp; rw [fdef]
+  case openm A =>
+    let indices := instance_indices Γ 0 x []
+    let insts := get_instances Γ indices
+    apply Or.inr; apply Exists.intro insts
+    apply @Red.inst #x x [] indices Γ insts
+    simp; simp; rw [fdef]; unfold Frame.is_openm; simp
+    simp; simp; simp
+  case type =>
+    replace h1 := h1 x
+    rw [fdef] at h1; unfold Frame.is_type at h1
+    simp at h1
+  case empty =>
+    unfold Frame.get_type at j2; simp at j2
+  all_goals (
+    apply Or.inl; apply @Val.app Γ #x x []
+    simp; simp; unfold Frame.is_stable_red
+    rw [fdef]
+  )
+case _ => apply Or.inl; apply Val.arrk
+case _ => apply Or.inl; apply Val.all
+case _ => apply Or.inl; apply Val.arr
+case _ Γ f A B a j1 j2 ih1 ih2 =>
+  have lem := classification_lemma j1; simp at lem
+  cases lem
+  case _ lem =>
+    have lem2 := types_are_values j1 lem
+    cases lem2
+    case app x sp q1 q2 =>
+      apply Or.inl; apply @Val.app Γ (f `@k a) x (sp ++ [(.kind, a)])
+      simp; rw [Option.bind_eq_some]; simp; apply q2
+      apply q1
+    all_goals (cases j1)
+  case _ lem =>
+    cases lem; case _ K lem =>
+    cases lem.2; cases lem.1
+case _ => apply Or.inl; apply Val.eq
+case _ Γ p A s R i B T e j1 j2 j3 j4 j5 j6 j7 j8 j9 j10 ih1 ih2 ih3 ih4 ih5 ih6 =>
+  replace ih2 := ih2 h1
+  cases ih2
+  case _ h2 =>
     apply Or.inr
+    unfold ValidHeadVariable at j5
+    unfold ValidHeadVariable at j6
+    cases j5; case _ w1 j5 =>
+    cases w1; case _ w1 sp1 =>
+    cases j6; case _ w2 j6 =>
+    cases w2; case _ w2 sp2 =>
+      simp at j5; simp at j6
+      cases h2
+      case _ x sp3 q2 q3 =>
+        generalize tstdef : prefix_equal sp1 sp3 = tst
+        cases tst
+        case _ =>
+          apply Exists.intro _
+          apply Red.ite_missed j5.1 (Eq.symm q3) q2 (Or.inr tstdef)
+        case _ ξ =>
+          cases (Nat.decEq w1 x)
+          case _ h =>
+            apply Exists.intro _
+            apply Red.ite_missed j5.1 (Eq.symm q3) q2 (Or.inl h)
+          case _ h =>
+            subst h; apply Exists.intro _
+            apply Red.ite_matched j5.1 (Eq.symm q3) (Eq.symm tstdef) j5.2
+      all_goals (cases j2; simp at j6)
+  case _ h2 =>
+    cases h2; case _ s' h2 =>
+      apply Or.inr
+      apply Exists.intro (List.map (fun x => p.ite x i e) s')
+      apply Red.ite_congr h2; rfl
+case _ Γ p A s R t B T j1 j2 j3 j4 j5 j6 j7 j8 j9 ih1 ih2 ih3 ih4 ih5 =>
+  replace ih2 := ih2 h1
+  cases ih2
+  case _ h2 =>
+    apply Or.inr
+    unfold ValidHeadVariable at j5
+    unfold ValidHeadVariable at j6
+    cases j5; case _ w1 j5 =>
+    cases w1; case _ w1 sp1 =>
+    cases j6; case _ w2 j6 =>
+    cases w2; case _ w2 sp2 =>
+      simp at j5; simp at j6
+      cases h2
+      case _ x sp3 q2 q3 =>
+        generalize tstdef : prefix_equal sp1 sp3 = tst
+        cases tst
+        case _ =>
+          apply Exists.intro _
+          apply Red.guard_missed j5.1 (Eq.symm q3) q2 (Or.inr tstdef)
+        case _ ξ =>
+          cases (Nat.decEq w1 x)
+          case _ h =>
+            apply Exists.intro _
+            apply Red.guard_missed j5.1 (Eq.symm q3) q2 (Or.inl h)
+          case _ h =>
+            subst h; apply Exists.intro [t.apply_spine ξ]
+            apply @Red.guard_matched p w1 sp1 s sp3 ξ Γ t
+            apply j5.1; apply Eq.symm q3
+            apply Eq.symm tstdef
+      all_goals (cases j2; simp at j6)
+  case _ h2 =>
+    cases h2; case _ s' h2 =>
+      apply Or.inr
+      apply Exists.intro (List.map (fun x => p.guard x t) s')
+      apply Red.guard_congr h2; rfl
+case _ => apply Or.inl; apply Val.lam
+case _ Γ f A B a B' j1 j2 j3 ih1 ih2 =>
+  replace ih1 := ih1 h1
+  cases ih1
+  case _ h2 =>
+    cases h2
+    case app x sp q1 q2 =>
+      apply Or.inl; apply @Val.app Γ (f `@ a) x (sp ++ [(.term, a)])
+      simp; rw [Option.bind_eq_some]; simp; apply q2
+      apply q1
+    case lam =>
+      apply Or.inr; apply Exists.intro _
+      apply Red.beta
+    all_goals (cases j1)
+  case _ h2 =>
+    cases h2; case _ f' h2 =>
+      apply Or.inr; apply Exists.intro (List.map (· `@ a) f')
+      apply Red.app_congr h2 rfl
+case _ => apply Or.inl; apply Val.lamt
+case _ Γ f A B a B' j1 j2 j3 ih1 ih2 =>
+  replace ih1 := ih1 h1
+  cases ih1
+  case _ h2 =>
+    cases h2
+    case app x sp q1 q2 =>
+      apply Or.inl; apply @Val.app Γ (f `@t a) x (sp ++ [(.type, a)])
+      simp; rw [Option.bind_eq_some]; simp; apply q2
+      apply q1
+    case lamt =>
+      apply Or.inr; apply Exists.intro _
+      apply Red.betat
+    all_goals (cases j1)
+  case _ h2 =>
+    cases h2; case _ f' h2 =>
+      apply Or.inr; apply Exists.intro (List.map (· `@t a) f')
+      apply Red.appt_congr h2 rfl
+case _ Γ t A c B j1 j2 ih1 ih2 =>
+  apply Or.inr
+  replace ih2 := ih2 h1
+  cases ih2
+  case _ h2 =>
+    have lem := refl_is_val j2 h2
+    cases lem; case _ e1 e2 =>
+      subst e1; subst e2
+      apply Exists.intro _
+      apply Red.cast
+  case _ h2 =>
+    cases h2; case _ c' h2 =>
+      apply Exists.intro (List.map (t ▹ ·) c')
+      apply Red.cast_congr h2 rfl
+case _ => apply Or.inl; apply Val.refl
+case sym Γ η A B ηJ ηs =>
+  apply Or.inr
+  cases ηs h1;
+  case _ h =>
+    have x := refl_is_val ηJ h;
+    have xeqrefl := x.left;
+    have aeqB := x.right; subst xeqrefl;
     have reds : ∃ t', Red Γ (sym! refl! A) t' := Exists.intro [refl! A] (@Red.sym Γ A);
     apply reds;
   case _ ηreds => cases ηreds; case _ w h =>
-    apply Or.inr;
     generalize tlp : List.map (sym! ·) w = tl' at *; symm at tlp;
     have reds : ∃ t', Red Γ (sym! η) t' := Exists.intro tl' (Red.sym_congr h tlp);
     apply reds;
 
 case seq Γ η1 A B η2 C η1J η2J η1s η2s =>
-  cases (η2s wΓ ntype);
+  apply Or.inr; cases (η2s h1);
   case _ h =>
-    have η2refp := refl_is_val ntype η2J h;
-    have η2refl := η2refp.1; cases (η1s wΓ ntype);
+    have η2refp := refl_is_val η2J h;
+    have η2refl := η2refp.1; cases (η1s h1);
     case _ h =>
-      have η1refp := refl_is_val ntype η1J h;
+      have η1refp := refl_is_val η1J h;
       have η1refl := η1refp.1; have aeqB := η1refp.2; have BeqC := η2refp.2
-      subst η1refl; subst η2refl;
-      apply Or.inr; subst aeqB;
+      subst η1refl; subst η2refl; subst aeqB;
       have reds : ∃ t', Red Γ ((refl! A) `; (refl! A)) t' := Exists.intro [refl! A] Red.seq;
-      apply reds
+      apply reds;
     case _ h => cases h; case _ w h =>
-      apply Or.inr;
       generalize tlp : List.map (· `; η2) w = tl' at *; symm at tlp;
       have reds : ∃ t', Red Γ (η1 `; η2) t' := Exists.intro tl' (Red.seq_congr1 h tlp);
       apply reds
   case _ h => cases h; case _ w h =>
-    apply Or.inr;
     generalize tlp : List.map (η1 `; ·) w = tl' at *; symm at tlp;
     have reds : ∃ t', Red Γ (η1 `; η2) t' := Exists.intro tl' (Red.seq_congr2 h tlp);
     apply reds
 
 case appc Γ A K1 K2 B η1 C D η2 aK bK η1J cJ dJ η2J _ _ η1s _ _ η2s  =>
-  -- check if η1 reduces or η2 reduces if both are values then reduce to refl
-  cases (η2s wΓ ntype);
+  apply Or.inr;
+  cases (η2s h1);
   case _ h =>
-    have η2refp := refl_is_val ntype η2J h;
-    have η2refl := η2refp.1; cases (η1s wΓ ntype);
+    have η2refp := refl_is_val η2J h;
+    have η2refl := η2refp.1; cases (η1s h1);
     case _ h =>
-      have η1refp := refl_is_val ntype η1J h;
-      have η1refl := η1refp.1; -- have aeqB := η1refp.2; have BeqC := η2refp.2
+      have η1refp := refl_is_val η1J h;
+      have η1refl := η1refp.1;
       subst η1refl; subst η2refl;
-      apply Or.inr;
       have reds : ∃ t', Red Γ ((refl! A) `@c (refl! C)) t' := Exists.intro [refl! (A `@k C)] Red.appc;
       apply reds
     case _ h => cases h; case _ w h =>
-      apply Or.inr;
       generalize tlp : List.map (· `@c η2) w = tl' at *; symm at tlp;
       have reds : ∃ t', Red Γ (η1 `@c η2) t' := Exists.intro tl' (Red.appc_congr1 h tlp);
       apply reds
   case _ h => cases h; case _ w h =>
-    apply Or.inr;
     generalize tlp : List.map (η1 `@c ·) w = tl' at *; symm at tlp;
     have reds : ∃ t', Red Γ (η1 `@c η2) t' := Exists.intro tl' (Red.appc_congr2 h tlp);
     apply reds
 
+
 case arrowc Γ A B η1 C D η2 _ _ η1J _ _ η2J _ _ η1s _ _ η2s =>
-  cases η2s (Judgment.wfempty wΓ) (DeclCtx.consempty ntype);
+  apply Or.inr; cases η2s (weaken_ctx_empty h1)
   case _ h =>
-    have ntype' : DeclCtx (Frame.empty :: Γ) := DeclCtx.consempty ntype;
-    have η2refp := refl_is_val ntype' η2J h;
-    have η2refl := η2refp.1; cases (η1s wΓ ntype);
+    have η2refp := refl_is_val η2J h;
+    have η2refl := η2refp.1; cases (η1s h1);
     case _ h =>
-      have η1refp := refl_is_val ntype η1J h;
+      have η1refp := refl_is_val η1J h;
       have η1refl := η1refp.1;
       subst η1refl; subst η2refl;
-      apply Or.inr;
       have reds : ∃ t', Red Γ (refl!(A) -c> refl! C) t' := Exists.intro [(refl! (A -t> C))] Red.arrowc;
       apply reds
     case _ h => cases h; case _ w h =>
-      apply Or.inr;
       generalize tlp : List.map (· -c> η2) w = tl' at *; symm at tlp;
       have reds : ∃ t', Red Γ (η1 -c> η2) t' := Exists.intro tl' (Red.arrowc_congr1 h tlp);
       apply reds
   case _ h => cases h; case _ w h =>
-    apply Or.inr;
     generalize tlp : List.map (η1 -c> ·) w = tl' at *; symm at tlp;
     have reds : ∃ t', Red Γ (η1 -c> η2) t' := Exists.intro tl' (Red.arrowc_congr2 h tlp);
     apply reds
 
 case fst Γ A _ _ _ η C _ _ _ ηJ _ _ ηs =>
-  cases (ηs wΓ ntype);
+  apply Or.inr; cases (ηs h1);
   case inl h =>
-    have ηrp := refl_is_val ntype ηJ h; have ηrfl := ηrp.1; subst ηrfl;
-    apply Or.inr;
+    have ηrp := refl_is_val ηJ h; have ηrfl := ηrp.1; subst ηrfl;
     have reds : ∃ t', Red Γ ((refl! (A `@k C)).!1) t' := Exists.intro [refl! A] Red.fst;
     apply reds;
   case inr h => cases h; case _ w h =>
-    apply Or.inr;
     generalize tlp : List.map (·.!1) w = tl' at *; symm at tlp;
     have reds : ∃ t', Red Γ (η.!1) t' := Exists.intro tl' (Red.fst_congr h tlp);
     apply reds
 
 case snd Γ _ C _ η A _ _ _ _ ηJ _ _ _ ηs =>
-  cases (ηs wΓ ntype);
+  apply Or.inr;
+  cases (ηs h1);
   case inl h =>
-    have ηrp := refl_is_val ntype ηJ h; have ηrfl := ηrp.1; subst ηrfl;
-    apply Or.inr;
+    have ηrp := refl_is_val ηJ h; have ηrfl := ηrp.1; subst ηrfl;
     have reds : ∃ t', Red Γ ((refl! (A `@k C)).!2) t' := Exists.intro [refl! C] Red.snd;
     apply reds;
   case inr h => cases h; case _ w h =>
-    apply Or.inr;
     generalize tlp : List.map (·.!2) w = tl' at *; symm at tlp;
     have reds : ∃ t', Red Γ (η.!2) t' := Exists.intro tl' (Red.snd_congr h tlp);
     apply reds
 
 case _ Γ K A B η allAJ allBJ ηJ _ _ ts =>
   cases allAJ; case _ kkind _ =>
-  have ts := ts (Judgment.wfkind kkind wΓ) (DeclCtx.conskind ntype);
-  cases ts;
+  have ts' : Val (Frame.kind K :: Γ) η ∨ ∃ t', Red (Frame.kind K :: Γ) η t' := ts (weaken_ctx_kind h1)
+  apply Or.inr;
+  cases ts';
   case inr h => cases h; case _ w h =>
-    simp_all;
-    apply Or.inr;
     generalize tlp : List.map (∀c[K]·) w = tl' at *; symm at tlp;
     have reds : ∃ t', Red Γ (∀c[K] η) t' := Exists.intro tl' (Red.allc_congr h tlp);
     apply reds
   case inl h =>
-    have ηrp := refl_is_val (DeclCtx.conskind ntype) ηJ h; have ηrfl := ηrp.1; subst ηrfl;
-    apply Or.inr;
+    have ηrp := refl_is_val ηJ h; have ηrfl := ηrp.1; subst ηrfl;
     have reds : ∃ t', Red Γ ((∀c[K] refl! A)) t' := Exists.intro [refl! (∀[K]A)] Red.allc;
     apply reds;
 
 case _ Γ η1 K A B C D η2 _ _ η1J CKJ _ η2J _ _ η1s _ _ η2s =>
-  cases (η2s wΓ ntype);
+  apply Or.inr;
+  cases (η2s h1);
   case _ h =>
-    have η2refp := refl_is_val ntype η2J h;
-    have η2refl := η2refp.1; cases (η1s wΓ ntype);
+    have η2refp := refl_is_val η2J h;
+    have η2refl := η2refp.1; cases (η1s h1);
     case _ h =>
-      have η1refp := refl_is_val ntype η1J h;
+      have η1refp := refl_is_val η1J h;
       have η1refl := η1refp.1;
       subst η1refl; subst η2refl;
-      apply Or.inr;
       have reds : ∃ t', Red Γ (refl!(∀[K] A) `@c[refl! C]) t' := Exists.intro [refl! (A β[ C ])] Red.apptc;
       apply reds
     case _ h => cases h; case _ w h =>
-      apply Or.inr;
       generalize tlp : List.map (· `@c[η2]) w = tl' at *; symm at tlp;
       have reds : ∃ t', Red Γ (η1 `@c[η2]) t' := Exists.intro tl' (Red.apptc_congr1 h tlp);
       apply reds
   case _ h => cases h; case _ w h =>
-    apply Or.inr;
     generalize tlp : List.map (η1 `@c[·]) w = tl' at *; symm at tlp;
     have reds : ∃ t', Red Γ (η1 `@c[η2]) t' := Exists.intro tl' (Red.apptc_congr2 h tlp);
     apply reds
+
+theorem progress :
+  (∀ x, ¬ Γ.is_type x) ->
+  Γ ⊢ t : A ->
+  Val Γ t ∨ (∃ t', Red Γ t t')
+:= by
+intro h j
+apply progress_lemma h j
