SystemFD/Metatheory.lean
@@ -1,2 +1,0 @@
-import SystemFD.Metatheory.Preservation
-import SystemFD.Metatheory.Progress2
