SystemFD/Metatheory/ProgressOld.lean
@@ -1,0 +1,812 @@
+
+import SystemFD.Term
+import SystemFD.Ctx
+import SystemFD.Judgment
+import SystemFD.Metatheory.Classification
+import SystemFD.Metatheory.Inversion
+import SystemFD.Reduction
+
+inductive Val : Ctx Term -> Term -> Prop where
+  | app : t.neutral_form = .some (n, ts)
+        -> (Γ.is_stable_red n)
+        -> Val Γ t
+  | appk : Val Γ (f `@k a)
+  | lam :  Val Γ (`λ[a] b)
+  | lamt : Val Γ (Λ[A] b)
+  | refl : Val Γ (refl! _)
+  | star : Val Γ ★
+  | arr :  Val Γ (A -t> B)
+  | arrk : Val Γ (A -k> B)
+  | all : Val Γ (∀[A]B)
+  | eq : Val Γ (A ~ B)
+
+
+theorem flip_eq : Γ ⊢ (A ~ B) : ★ -> Γ ⊢ (B ~ A) : ★ := by
+intros h; cases h; case _ k AJ BJ => apply Judgment.eq k BJ AJ
+
+theorem not_neutral_form_shape : Val Γ t ->
+        t.neutral_form = .some (n, ts)
+        -> ¬ ((t = `λ[A] b)
+            ∨ (t = Λ[A] b)
+            ∨ t = .letterm A t' b
+            ∨ t = .guard p s b
+            ∨ t = .ite p s b c
+            ∨ t = .kind
+            ∨ t = .type
+            -- ∨ t = refl! A
+            -- ∨ t = sym! η
+            ) := by
+intros tnf; induction t;
+any_goals (solve | simp_all)
+
+def DeclCtx (Γ : Ctx Term) : Prop := (∀ n,  ¬ Γ.is_type n)
+namespace DeclCtx
+theorem consempty : DeclCtx Γ -> DeclCtx (.empty :: Γ) := by
+  intros dctx; induction Γ;
+  case _ =>
+    unfold DeclCtx; intro n xx; unfold Ctx.is_type at xx; unfold Frame.is_type at xx;
+    cases n;
+    case _ =>
+      simp_all; unfold Frame.apply at xx; simp at xx;
+    case _ => simp at xx; unfold Frame.apply at xx; simp at xx
+  case _ hf tl ih =>
+    unfold DeclCtx; unfold DeclCtx at dctx;
+    unfold Ctx.is_type;
+    sorry
+theorem conskind : DeclCtx Γ -> DeclCtx (.kind t :: Γ) := by sorry
+
+end DeclCtx
+
+theorem no_lam_bindings : (DeclCtx Γ) -> (∀ x, ¬ (Γ d@ x = .type T)) := by
+intro dctx x h;
+have xx := @dctx x; simp at xx; rw[h] at xx; unfold Frame.is_type at xx; simp_all;
+
+theorem dt_is_dt {Γ : Ctx Term}: Γ d@x = Frame.datatype t -> (Γ d@ x).is_datatype := by
+intros dt; simp_all; unfold Frame.is_datatype; simp;
+
+theorem dt_is_stable {Γ : Ctx Term}{x : Nat}: Γ d@ x = Frame.datatype t -> Frame.is_stable_red (Γ d@ x) := by
+intros dt; unfold Frame.is_stable_red; rw [dt];
+
+theorem opent_is_stable {Γ : Ctx Term}: Γ d@x = Frame.opent t -> Frame.is_stable_red (Γ d@ x) := by
+intros dt; unfold Frame.is_stable_red; rw [dt];
+
+theorem apptneqrefl : ¬ ((f `@t a) = (refl! A)) := by simp_all
+theorem appneqrefl : ¬ ((f `@ a) = (refl! A)) := by simp_all
+
+theorem openm_no_stable {Γ : Ctx Term}{n : Nat} :
+  Frame.is_openm (Γ d@ n) = true -> ¬ (Frame.is_stable_red (Γ d@ n)) := by
+intros om; simp_all; unfold Frame.is_openm at om; split at om;
+case _ => unfold Frame.is_stable_red; simp_all;
+case _ => simp_all
+
+theorem stable_no_reduce : t.neutral_form = .some (n, sp) -> Γ.is_stable_red n = true -> ¬ ∃ t', Red Γ t t' := by
+intros tnf nstable x; cases x;
+  case _ w h =>
+  simp_all; induction h generalizing n sp;
+  any_goals (solve | simp_all)
+  case _ Γ _ _ _ _ om _ _ nstable =>
+    have n_not_stable := openm_no_stable om;
+    simp_all;
+  case _ hnf idx =>
+    unfold Frame.is_stable_red at nstable; symm at hnf;
+    have uniq' := Term.unique_neutral_form hnf tnf; have uniq := uniq'.1;
+    subst uniq; rw [<-idx] at nstable; simp_all
+  case _ f _ _ a _ _ ih =>
+    simp_all; rw[Option.bind_eq_some] at tnf;
+    cases tnf; case _ w h =>
+      have fa_spine := @Term.neutral_form_app f a w.fst w.snd h.1;
+      have f_spine := Term.neutral_form_app_rev fa_spine;
+      have xx := @ih w.1 w.2 f_spine; simp at h;
+      have wfst := And.left (And.right h); symm at wfst;
+      subst wfst; simp_all;
+  case _ ih =>
+    simp_all; rw [Option.bind_eq_some] at tnf;
+    cases tnf; case _ f _ _ a _ _ w h =>
+      have fa_spine := @Term.neutral_form_appt f a w.fst w.snd h.1;
+      have f_spine := Term.neutral_form_appt_rev fa_spine;
+      have xx := @ih w.1 w.2 f_spine; simp at h;
+      have wfst := And.left (And.right h); symm at wfst;
+      subst wfst; simp_all;
+
+@[simp]
+abbrev ValueNoSteps : (v : JudgmentVariant) -> (Γ : Ctx Term)  -> (JudgmentArgs v) -> Prop
+| .prf => λ Γ => λ(t , _) => Val Γ t -> ¬ ∃ t', Red Γ t t'
+| .wf  => λ _ => λ () => true
+
+
+theorem val_no_red :
+  DeclCtx Γ ->
+  Judgment v Γ ix ->
+  ValueNoSteps v Γ ix
+  := by
+intros dctx tJ; have wΓ := judgment_ctx_wf tJ;
+induction tJ;
+any_goals(solve | simp_all)
+all_goals(intro vt treds; cases treds; cases vt; simp_all)
+case _ h =>
+  cases h;
+  case _ => simp_all
+  case _ => simp_all
+case _ h _ _ =>
+  cases h;
+  case _  n _ x_stable _ _ _ _ _ x_openm _ _ nnf _ =>
+    symm at nnf; have nnf' := @Term.var_neutral_form n; rw[nnf'] at nnf; injection nnf with nnf; simp at nnf;
+    have x_n := nnf.1; rw[<-x_n] at x_openm;
+    have x_not_stable := Frame.is_openm_implies_not_is_stable_red x_openm; contradiction;
+  case _ n' _ x_stable _ _ n _ _ x_term nnf =>
+    symm at nnf; have nnf' := @Term.var_neutral_form n'; rw[nnf'] at nnf; simp at nnf;
+    have n_n := nnf.1; rw[n_n] at x_stable; rw[<-x_term] at x_stable;
+    unfold Frame.is_stable_red at x_stable; simp at x_stable;
+case _ h =>
+  cases h;
+  case _ h _ => cases h
+  case _ h => cases h
+case _ h =>
+  cases h;
+  case _ h _ => cases h
+  case _ h => cases h
+case _ h =>
+  cases h
+  case _ h _ => cases h
+  case _ h => cases h
+case _ h =>
+  rw [Option.bind_eq_some] at h; cases h
+  case _ h _ _ _ =>
+    cases h;
+    case _ _ x_stable _ _ _ _ _ _ x_openm _ _ hh _ =>
+      simp_all; have hh := hh.1; subst hh; simp_all;
+      have x_not_stable := Frame.is_openm_implies_not_is_stable_red x_openm; contradiction;
+    case _ Γ f _ _ arg _ _ n ts _ _ x_stable w fnfp _ x sp _ x_term hh =>
+      have fnf := fnfp.2;
+      injection fnf with fnf;
+      have weqx : w.fst = n := by simp_all;
+      have tseqw :  w.snd ++ [(.kind, arg)]= ts := by simp_all;
+      symm at tseqw;
+      symm at hh;
+      subst weqx; subst tseqw;
+      have xx := Term.neutral_form_appk_rev_exists hh; cases xx;
+      case _ fnfp =>
+        have hh := fnfp.2; subst hh; simp_all;
+        have hh1 := hh.1; have hh2 := hh.2;
+        have xterm : Γ.is_term x = true := by simp; unfold Frame.is_term; rw[<-x_term];
+        have x_not_stable := Frame.is_term_implies_not_is_stable_red xterm; apply (x_not_stable x_stable);
+case _ Γ f _ _ a fj _ _ _ _ h =>
+  cases h;
+  case _ =>
+    have lem := classification_lemma fj; simp at lem;
+    cases lem;
+    case _ => simp_all; sorry
+    case _ h => cases h; case _ w h => sorry
+
+  case _ T x sp t x_term fanf =>
+    symm at fanf; have fanf := Term.neutral_form_appk_rev_exists fanf;
+    cases fanf; case _ fsp fanf =>
+    symm at x_term; symm at fanf;
+    have xx := ctx_get_term_well_typed wΓ x_term;
+    sorry
+    -- have xx' := ctx_get_term_type_kind wΓ x_term;
+    -- have lem := classification_lemma xx.1; simp at lem; cases lem;
+    -- case _ h => subst h; cases xx'.2;
+    -- case _ h =>
+    --   cases h;
+    --   case _ h => have uniq := uniqueness_of_types xx'.2 h; simp_all;
+    --   case _ h => sorry
+          -- cases h; case _ h =>
+          --   have uniq := uniqueness_of_types xx' h.2; subst uniq;
+          --   have f_form := Term.neutral_form_law fp; subst f_form; simp_all;
+          --   case _ fj => sorry
+case _ h =>
+  cases h;
+  case _ => simp_all
+  case _ => simp_all
+case _ h =>
+  cases h;
+  case _ => simp_all
+  case _ => simp_all
+case _ h' _ h =>
+  rw[Option.bind_eq_some] at h;
+  cases h'
+  case _ => simp_all;
+  case _ => sorry
+  case _ => sorry
+  case _ => sorry
+case _ h =>
+  cases h;
+  case _ => simp_all
+  case _ => simp_all
+case _ h' _ h =>
+  rw[Option.bind_eq_some] at h;
+  cases h; case _ fnf =>
+    cases h';
+    case _ => simp_all
+    case _ => simp_all; sorry
+    case _ => sorry
+    case _ => sorry
+case _ h =>
+  cases h;
+  case _ => simp_all
+  case _ => simp_all
+
+-- s is a value, cannot have a neutral form; datatype type, is impossible
+theorem term_neutral_form_datatype :
+  Val Γ t ->
+  t.neutral_form = .none ->
+  ValidHeadVariable T Γ.is_datatype ->
+  Γ ⊢ t : T ->
+  False := by
+intros tv nf vhv tJ;
+induction tv;
+any_goals (solve | simp_all)
+any_goals (solve | cases tJ; cases vhv; simp_all)
+case _ Γ f h =>
+  have lem := type_disjoint tJ; simp at lem;
+  unfold ValidHeadVariable at vhv;
+  sorry
+
+theorem term_neutral_form_opent :
+  Val Γ t ->
+  t.neutral_form = .none ->
+  ValidHeadVariable T Γ.is_opent ->
+  Γ ⊢ t : T ->
+  False := by
+intros tv nf vhv tJ;
+sorry
+
+
+theorem var_type_lemma :
+  Γ.is_stable_red n ->
+  Γ ⊢ (#n).apply_spine ts : (A ~ B)
+  -> False := by
+intros n_stable h; induction ts;
+case _ => simp_all; cases h; case _ wΓ ty => symm at ty;  apply (ctx_get_var_no_eq_type wΓ n_stable ty);
+case _ hd tl ih =>
+   sorry
+
+
+theorem var_well_typed :
+  Γ.is_stable_red n ->
+  Γ ⊢ #n : (A ~ B)
+  -> False := by
+intros n_stable tJ; cases tJ;
+case _ wΓ ty =>
+  symm at ty; apply (ctx_get_var_no_eq_type wΓ n_stable ty);
+
+theorem var_app_well_typed :
+  Γ.is_stable_red n ->
+  Γ ⊢ (#n `@ t) : (A ~ B)
+  -> False := by
+intros n_stable tJ;
+cases tJ;
+case _ nJ tJ eq =>
+  cases nJ;
+  case _ wΓ nty =>
+    symm at nty; induction Γ;
+    case _ => unfold Frame.get_type at nty; simp at nty
+    case _ hf tlf ih =>
+         unfold Ctx.is_stable_red at n_stable; unfold Frame.is_stable_red at n_stable; simp at n_stable;
+         sorry
+
+theorem refl_is_val : DeclCtx Γ -> Γ ⊢ η : (A ~ B)
+                    -> Val Γ η
+                    -> η = refl! A ∧ A = B := by
+intros dctx ηJ vη; induction vη;
+any_goals(solve | cases ηJ)
+case _ Γ t n ts tnf n_stable =>
+     symm at tnf; replace tnf := Term.neutral_form_law tnf;
+     subst tnf; exfalso; apply (var_type_lemma n_stable ηJ);
+case _ => cases ηJ; case _ fJ =>
+  have lem := classification_lemma fJ; simp at lem; cases lem;
+  case _ h => cases h; case _ h => have h := invert_eq_kind h; cases h;
+  case _ h => cases h; case _ h => simp_all; cases h.2; cases h.1
+case _ => cases ηJ; simp_all
+
+theorem ctor_uniqueness {Γ : Ctx Term}: (Γ.is_ctor x = true) -> (Γ.is_ctor y = false) -> x ≠ y := by
+intros xctor yctor xeqy ;
+induction Γ;
+case _ => simp_all
+case _ here there ih =>
+  unfold Ctx.is_ctor at xctor; unfold dnth at xctor;
+  split at xctor;
+  case _ => simp_all;
+  case _ =>
+    simp_all; subst xeqy;
+    unfold dnth at yctor; simp_all;
+  case _ =>
+    simp_all; subst xeqy;
+    unfold dnth at yctor; simp_all;
+
+theorem insttype_uniqueness {Γ : Ctx Term}: (Γ.is_insttype x = true) -> (Γ.is_insttype y = false) -> x ≠ y := by
+intros xinst yinst xeqy ;
+induction Γ;
+case _ => simp_all
+case _ here there ih =>
+  unfold Ctx.is_insttype at xinst; unfold dnth at xinst;
+  split at xinst;
+  case _ => simp_all;
+  case _ =>
+    simp_all; subst xeqy;
+    unfold dnth at yinst; simp_all;
+  case _ =>
+    simp_all; subst xeqy;
+    unfold dnth at yinst; simp_all;
+
+
+-- this is stupid
+theorem bool_implication (x : Bool) : x = false -> ¬ x = true :=
+by intro h; rw [h]; simp
+
+
+theorem head_cannot_be_empty :
+   DeclCtx Γ ->
+   Γ ⊢ t : T ->
+   .some (x, sp) = Term.neutral_form t ->
+   ¬ Γ d@ x  = .empty
+:= by
+intros dctx tJ tnf x_empty;
+induction sp
+case _ =>
+  simp_all;
+  have xx' := Term.neutral_form_law tnf; unfold Term.apply_spine at xx';
+  rw [<-xx'] at tJ;
+  cases tJ; case _ h => rw [x_empty] at h; unfold Frame.get_type at h; simp at h
+case _ ht tl ih =>
+  have xx := Term.neutral_form_law tnf;
+
+  sorry
+
+
+theorem unstable_var_steps :
+   (∀ n,  ¬ Γ.is_type n) ->
+   Γ ⊢ t : T ->
+   .some (x, sp) = Term.neutral_form t ->
+   (Γ.is_stable_red x = false) ->
+   ∃ t', Red Γ t t'
+:= by
+intros dctx tJ tnf x_not_stable;
+have x_not_stable := @bool_implication (Γ.is_stable_red x) x_not_stable;
+generalize xx : Γ d@ x = f;
+cases f;
+any_goals (solve | unfold Ctx.is_stable_red at x_not_stable
+                   rw [xx] at x_not_stable
+                   simp at x_not_stable
+                   unfold Frame.is_stable_red at x_not_stable
+                   simp at x_not_stable)
+case empty =>
+  have no_empty := (head_cannot_be_empty dctx tJ tnf);
+  exfalso; apply (no_empty xx)
+case type => have xx' := @dctx x; unfold Ctx.is_type at xx'; rw [xx] at xx'; unfold Frame.is_type at xx'; simp_all;
+case term lt =>
+  symm at xx; have reds := Red.letterm tnf xx;
+  apply Exists.intro [lt.apply_spine sp] reds;
+case openm =>
+   have om : (Γ d@ x).is_openm := by unfold Frame.is_openm; rw [xx];
+   generalize isp : instance_indices Γ 0 x [] = ιs at *; symm at isp;
+   generalize instsp : get_instances Γ ιs = insts at *; symm at instsp;
+   generalize instsp' : List.map (·.apply_spine sp) insts = insts' at *; symm at instsp';
+   apply (Exists.intro insts' (Red.inst tnf om isp instsp instsp'))
+
+@[simp]
+abbrev StepOrVal : (v : JudgmentVariant) -> (Γ : Ctx Term) -> (JudgmentArgs v) -> Prop
+| .prf => λ Γ => λ(t , _) => Val Γ t ∨ ∃ t', Red Γ t t'
+| .wf  => λ _ => λ () => true
+
+theorem progress :
+   ⊢ Γ -> (∀ n,  ¬ Γ.is_type n)
+  -> Judgment v Γ ix
+--------------------------------------
+  -> StepOrVal v Γ ix := by
+intros wΓ ntype j; induction j;
+any_goals (solve | simp_all)
+case _ Γ A t b _ _ _ _ _ _ _ ih _ =>
+  simp_all;
+  generalize tl' : [b β[ t ]] = t' at *; symm at tl';
+  have reds := @Red.letbeta Γ A t b; rw [<-tl']  at reds;
+  have ereds : ∃ t', Red Γ (.letterm A t b) t' := Exists.intro t' reds;
+  apply Or.inr ereds;
+
+case _ => simp_all; apply Or.inl Val.star;
+case var Γ x _ _ xTy ih =>
+  simp at ih;
+  unfold Frame.get_type at xTy; simp at xTy;
+  split at xTy;
+  any_goals (solve | simp_all)
+  case _ f _ x_is_kind => -- bogus case
+    simp_all; have xK := ctx_get_var_type wΓ x_is_kind;
+    have hh : (#x).neutral_form = .some (x, []) := Term.var_neutral_form;
+    have k_st_red : Γ.is_stable_red x := by simp; unfold Frame.is_stable_red; rw [x_is_kind]
+    apply Or.inl (Val.app hh k_st_red);
+  case _ f _ x_is_type =>
+    exfalso; have ntype' := ntype x; simp at ntype'; rw[x_is_type] at ntype';
+    unfold Frame.is_type at ntype'; simp at ntype';
+  case _ f _ x_is_datatype =>
+      simp_all; have x_is_stable := dt_is_stable x_is_datatype;
+      have hh : (#x).neutral_form = .some (x, []) := Term.var_neutral_form;
+      apply Or.inl;
+      apply Val.app hh x_is_stable;
+  case _ f t x_is_ctor =>
+    have xx : Frame.is_stable_red (Γ d@ x) := by unfold Frame.is_stable_red; rw[x_is_ctor];
+    have hh : (#x).neutral_form = .some (x, []) := Term.var_neutral_form;
+    apply Or.inl (Val.app hh xx)
+  case _ x_is_opent =>
+      have x_is_stable := opent_is_stable x_is_opent;
+      have hh : (#x).neutral_form = .some (x, []) := Term.var_neutral_form;
+      apply Or.inl;
+      apply Val.app hh x_is_stable;
+  case _ x_is_openm =>  -- steps inst
+    have nf  := @Term.var_neutral_form x; symm at nf;
+    have om : (Γ d@ x).is_openm := by unfold Frame.is_openm; rw [x_is_openm];
+    generalize isp : instance_indices Γ 0 x [] = ιs at *; symm at isp;
+    generalize instsp : get_instances Γ ιs = insts at *; symm at instsp;
+    generalize instsp' : List.map (·.apply_spine []) insts = insts' at *; symm at instsp';
+    apply Or.inr (Exists.intro insts' (Red.inst nf om isp instsp instsp'))
+  case _ x_is_insttype =>  -- value
+    have xx : Frame.is_stable_red (Γ d@ x) := by unfold Frame.is_stable_red; rw[x_is_insttype];
+    have hh : (#x).neutral_form = .some (x, []) := Term.var_neutral_form;
+    apply Or.inl (Val.app hh xx)
+  case _ A t x_frame =>  -- steps letterm
+    have nf : .some (x, []) = (#x).neutral_form := Term.var_neutral_form;
+    have x_is_term : .term A t = Γ d@ x := by symm at x_frame; apply x_frame
+    generalize tlp : [t.apply_spine []] = t' at *; symm at tlp;
+    have etl' : ∃ t', Red Γ (#x) t' := Exists.intro ([t.apply_spine []]) (Red.letterm nf x_is_term);
+    apply Or.inr etl'
+
+case _ => simp_all; apply Or.inl; apply Val.arrk
+case _ => simp_all; apply Or.inl; apply Val.all
+case _ => simp_all; apply Or.inl; apply Val.arr
+
+case appk fs as => simp_all;  apply Or.inl; apply Val.appk
+
+case _ => simp_all; apply Or.inl; apply Val.eq
+
+case ite Γ p A s _ i _ _ e _ sJ RJ _ vhvp vhvr stm _ tstar _ ps ss _ is _ es =>
+  cases vhvp; case _ pf h =>
+    have pnf := h.1; have hpctor := h.2;
+    have p_n := pf.1; have p_sp := pf.2;
+    generalize snf : s.neutral_form = xx at *; symm at snf;
+    cases xx;
+    case _ =>
+       cases (ss wΓ ntype)
+       case _ h => exfalso; symm at snf; apply (term_neutral_form_datatype h snf vhvr sJ)
+       case _ h => cases h; case _ w h =>
+          generalize tlp : List.map (Term.ite p · i e) w = tl' at *; symm at tlp;
+          have reds : ∃ t', Red Γ (.ite p s i e) t' := Exists.intro tl' (Red.ite_congr h tlp);
+          apply Or.inr reds
+    case _ sf =>
+       simp;
+       have s_sp := sf.2;
+       generalize sp : sf.1 = s_n at *; symm at sp;
+       generalize s_spp : sf.2 = s_sp at *; symm at s_spp;
+       generalize snctor : Γ.is_ctor s_n = p at *;
+       have s_form := Term.neutral_form_law snf; rw[<-s_spp] at s_form; rw[<-sp] at s_form;
+       cases p;
+       case _ => -- scrutinee is a not ctor headed but has a neutral form
+         generalize xx : Γ.is_stable_red s_n = x_is_stable;
+         cases x_is_stable;
+         case false =>
+           apply Or.inr; simp at xx; rw[sp] at xx;
+           have reds' := unstable_var_steps ntype sJ snf xx;
+           cases reds'; case _ w sreds =>
+           generalize tlp : List.map (Term.ite p · i e) w = tl at *; symm at tlp;
+           have reds : ∃ t', Red Γ (.ite p s i e) t' := Exists.intro tl (Red.ite_congr sreds tlp)
+           apply reds
+         case true =>
+           generalize xx' : Γ d@ s_n = f;
+           cases f;
+           any_goals (solve | unfold Ctx.is_stable_red at xx; rw [xx'] at xx; unfold Frame.is_stable_red at xx; simp at xx)
+           any_goals (solve | subst sp;
+                              have reds : ∃ t', Red Γ (.ite p s i e) t' :=
+                                Exists.intro [e] (Red.ite_missed pnf snf xx (Or.inl (ctor_uniqueness hpctor snctor)));
+                              apply Or.inr; apply reds)
+
+       case _ =>
+          have check := Nat.decEq pf.fst sf.fst;
+          cases check;
+          case _ h =>
+            have s_is_stable : Γ.is_stable_red sf.fst := by rw[sp] at snctor; apply Frame.is_ctor_implies_is_stable_red snctor;
+            have reds : ∃ t', Red Γ (.ite p s i e) t' := Exists.intro [e] (Red.ite_missed pnf snf s_is_stable (Or.inl h));
+            apply Or.inr; apply reds;
+          case _ h =>
+            generalize comp_prefix : prefix_equal pf.snd sf.snd = h at *;
+            cases h
+            case _ h =>
+              have s_is_stable : Γ.is_stable_red sf.fst := by rw[sp] at snctor; apply Frame.is_ctor_implies_is_stable_red snctor;
+              have reds : ∃ t', Red Γ (.ite p s i e) t' :=
+                   Exists.intro [e] (Red.ite_missed pnf snf s_is_stable (Or.inr comp_prefix));
+              apply Or.inr; apply reds;
+            case _ h' =>
+              symm at comp_prefix;
+              have sfp : sf = (sf.fst , sf.snd) := by simp_all;
+              rw [sfp] at snf; rw[<-h] at snf;
+              have reds : ∃ t', Red Γ (.ite p s i e) t' :=
+                Exists.intro [i.apply_spine h'] (Red.ite_matched pnf snf comp_prefix hpctor);
+              apply Or.inr; apply reds;
+
+case guard Γ p A s R t _ _ pJ sJ _ _ vhvp vhvr _ _ _  ps ss _ _ _  =>
+  cases vhvp; case _ pf h =>
+    have pnf := h.1; have hpctor := h.2;
+    have p_n := pf.1; have p_sp := pf.2;
+    generalize snf : s.neutral_form = xx at *; symm at snf;
+    cases xx;
+    case _ =>
+       cases (ss wΓ ntype)
+       case _ h => exfalso; symm at snf; apply (term_neutral_form_opent h snf vhvr sJ)
+       case _ h => cases h; case _ w h =>
+          generalize tlp : List.map (Term.guard p · t) w = tl' at *; symm at tlp;
+          have reds : ∃ t', Red Γ (.guard p s t) t' := Exists.intro tl' (Red.guard_congr h tlp);
+          apply Or.inr reds
+    case _ sf =>
+       simp
+       generalize snctor : Γ.is_insttype sf.fst = p at *;
+       generalize sp : sf.1 = s_n at *; symm at sp;
+       generalize s_spp : sf.2 = s_sp at *; symm at s_spp;
+       have s_form := Term.neutral_form_law snf; rw[<-s_spp] at s_form; rw[<-sp] at s_form;
+       cases p;
+       case _ =>   -- scrutinee is a not a opentype headed but has a neutral form
+         generalize xx : Γ.is_stable_red s_n = x_is_stable;
+         cases x_is_stable;
+         case false =>
+           apply Or.inr; simp at xx; rw[sp] at xx;
+           have reds' := unstable_var_steps ntype sJ snf xx;
+           cases reds'; case _ w sreds =>
+           generalize tlp : List.map (Term.guard p · t) w = tl at *; symm at tlp;
+           have reds : ∃ t', Red Γ (Term.guard p s t) t' := Exists.intro tl (Red.guard_congr sreds tlp)
+           apply reds
+         case true =>
+           generalize xx' : Γ d@ s_n = f;
+           cases f;
+           any_goals (solve | unfold Ctx.is_stable_red at xx; rw [xx'] at xx; unfold Frame.is_stable_red at xx; simp at xx)
+           any_goals (solve | subst sp;
+                              have reds : ∃ t', Red Γ (.guard p s t) t' :=
+                                Exists.intro [] (Red.guard_missed pnf snf xx (Or.inl (insttype_uniqueness hpctor snctor)));
+                              apply Or.inr; apply reds)
+       case _ =>
+          have check := Nat.decEq pf.fst sf.fst;
+          cases check;
+          case _ h =>
+            have s_is_stable : Γ.is_stable_red sf.fst := by rw[sp] at snctor; apply Frame.is_insttype_implies_is_stable_red snctor;
+            have reds : ∃ t', Red Γ (.guard p s t) t' := Exists.intro [] (Red.guard_missed pnf snf s_is_stable (Or.inl h));
+            apply Or.inr; apply reds; -- sorry
+          case _ h =>
+            generalize comp_prefix : prefix_equal pf.snd sf.snd = h at *;
+            cases h
+            case _ h =>
+              have s_is_stable : Γ.is_stable_red sf.fst := by rw[sp] at snctor; apply Frame.is_insttype_implies_is_stable_red snctor;
+              have reds : ∃ t', Red Γ (.guard p s t) t' :=
+                   Exists.intro [] (Red.guard_missed pnf snf s_is_stable (Or.inr comp_prefix));
+              apply Or.inr; apply reds;
+            case _ h' =>
+              symm at comp_prefix;
+              have sfp : sf = (sf.fst , sf.snd) := by simp_all;
+              rw [sfp] at snf; rw[<-h] at snf;
+              have reds : ∃ t', Red Γ (.guard p s t) t' :=
+                Exists.intro [t.apply_spine h'] (Red.guard_matched pnf snf comp_prefix);
+              apply Or.inr; apply reds;
+
+case _ _ A t _ _ _ _ _ _ _ => apply Or.inl Val.lam
+
+case app Γ f A B a B' fJ aJ _ fs as =>
+  have fs' := fs wΓ ntype;
+  cases fs'
+  case inl h => -- f is value
+    cases h;
+    case app n ts n_stable fnf =>
+       have fanf := @Term.neutral_form_app f a n ts fnf;
+       apply Or.inl (Val.app fanf n_stable);
+    case lam A B =>
+      apply Or.inr;
+      have reds : ∃ t', Red Γ ((`λ[A]B) `@ a) t' := Exists.intro [B β[ a ]] (@Red.beta Γ A B a);
+      apply reds
+    case lamt  => have xx := lamt_typing_unique fJ; cases xx; case _ w h => cases h;
+    case refl => have xx := refl_typing_unique fJ; cases xx
+    case _ => cases fJ; case _ fJ' =>
+      have lem := classification_lemma fJ'; simp at lem; cases lem;
+      case _ h => cases h; case _ h => cases h;
+      case _ h => cases h; case _ h => cases h.2; cases h.1;
+    case _ => have fJ' := Judgment.ax wΓ; have u := uniqueness_of_types fJ fJ'; cases u;
+    case _ => cases fJ
+    case _ => cases fJ;
+    case _ => cases fJ
+    case _ => cases fJ
+
+  case inr h => cases h; case _ w h => -- f steps
+    generalize tlp : List.map (· `@ a) w = tl' at *; symm at tlp;
+    have reds : ∃ t', Red Γ (f `@ a) t' := Exists.intro tl' (Red.app_congr h tlp);
+    apply Or.inr reds
+
+case _ _ A t _ _ _ _ _ _ _ => apply Or.inl Val.lamt
+
+case appt Γ f _ _ a _ fJ aJ _ fs as =>
+  cases fs wΓ ntype;
+  case inr h => cases h; case _ w h =>
+      apply Or.inr;
+      generalize tlp : List.map (· `@t a) w = tl' at *; symm at tlp;
+      have reds : ∃ t', Red Γ (f `@t a) t' := Exists.intro tl' (Red.appt_congr h tlp);
+      apply reds;
+  case inl h =>
+    cases h;
+    case app n ts n_stable fnf =>
+      have fanf := @Term.neutral_form_appt f a n ts fnf
+      apply Or.inl;
+      apply (Val.app fanf n_stable);
+    case lam => have xx := lam_typing_unique fJ; cases xx; simp_all;
+    case lamt a' b =>
+      apply Or.inr;
+      have reds : ∃ t', Red Γ ((Λ[a']b) `@t a) t' := Exists.intro [b β[ a ]] (@Red.betat Γ a' b a);
+      apply reds
+    case refl => have xx := refl_typing_unique fJ; cases xx
+    case _ => cases fJ; case _ fJ' =>
+      have lem := classification_lemma fJ'; simp at lem; cases lem;
+      case _ h => cases h; case _ h => cases h;
+      case _ h => cases h; case _ h => cases h.2; cases h.1;
+    case _ => have fJ' := Judgment.ax wΓ; have xx := uniqueness_of_types fJ fJ'; cases xx
+    case _ => cases fJ
+    case _ => cases fJ
+    case _ => cases fJ
+    case _ => cases fJ
+
+case _ Γ t A η B tJ ηJ ts cs =>
+  cases (cs wΓ ntype);
+  case _ h =>
+      have ηreflp := @refl_is_val Γ η A B ntype ηJ h;
+      have ηrefl := ηreflp.1;
+      subst ηrefl; apply Or.inr;
+      have reds : ∃ t', Red Γ (t ▹ refl! A) t' := Exists.intro [t] Red.cast;
+      apply reds
+  case _ h => cases h; case _ w h =>
+      apply Or.inr
+      generalize tlp : List.map (t ▹ ·) w = tl' at *; symm at tlp;
+      have reds : ∃ t', Red Γ (t ▹ η) t' := Exists.intro tl' (Red.cast_congr h tlp);
+      apply reds;
+
+case _ => apply Or.inl Val.refl
+case sym Γ η A B ηJ ηs =>
+  cases ηs wΓ ntype;
+  case _ h =>
+    have x := refl_is_val ntype ηJ h;
+    have xeqrefl := x.left;
+    have aeqB := x.right;
+    subst xeqrefl;
+    apply Or.inr
+    have reds : ∃ t', Red Γ (sym! refl! A) t' := Exists.intro [refl! A] (@Red.sym Γ A);
+    apply reds;
+  case _ ηreds => cases ηreds; case _ w h =>
+    apply Or.inr;
+    generalize tlp : List.map (sym! ·) w = tl' at *; symm at tlp;
+    have reds : ∃ t', Red Γ (sym! η) t' := Exists.intro tl' (Red.sym_congr h tlp);
+    apply reds;
+
+case seq Γ η1 A B η2 C η1J η2J η1s η2s =>
+  cases (η2s wΓ ntype);
+  case _ h =>
+    have η2refp := refl_is_val ntype η2J h;
+    have η2refl := η2refp.1; cases (η1s wΓ ntype);
+    case _ h =>
+      have η1refp := refl_is_val ntype η1J h;
+      have η1refl := η1refp.1; have aeqB := η1refp.2; have BeqC := η2refp.2
+      subst η1refl; subst η2refl;
+      apply Or.inr; subst aeqB;
+      have reds : ∃ t', Red Γ ((refl! A) `; (refl! A)) t' := Exists.intro [refl! A] Red.seq;
+      apply reds
+    case _ h => cases h; case _ w h =>
+      apply Or.inr;
+      generalize tlp : List.map (· `; η2) w = tl' at *; symm at tlp;
+      have reds : ∃ t', Red Γ (η1 `; η2) t' := Exists.intro tl' (Red.seq_congr1 h tlp);
+      apply reds
+  case _ h => cases h; case _ w h =>
+    apply Or.inr;
+    generalize tlp : List.map (η1 `; ·) w = tl' at *; symm at tlp;
+    have reds : ∃ t', Red Γ (η1 `; η2) t' := Exists.intro tl' (Red.seq_congr2 h tlp);
+    apply reds
+
+case appc Γ A K1 K2 B η1 C D η2 aK bK η1J cJ dJ η2J _ _ η1s _ _ η2s  =>
+  -- check if η1 reduces or η2 reduces if both are values then reduce to refl
+  cases (η2s wΓ ntype);
+  case _ h =>
+    have η2refp := refl_is_val ntype η2J h;
+    have η2refl := η2refp.1; cases (η1s wΓ ntype);
+    case _ h =>
+      have η1refp := refl_is_val ntype η1J h;
+      have η1refl := η1refp.1; -- have aeqB := η1refp.2; have BeqC := η2refp.2
+      subst η1refl; subst η2refl;
+      apply Or.inr;
+      have reds : ∃ t', Red Γ ((refl! A) `@c (refl! C)) t' := Exists.intro [refl! (A `@k C)] Red.appc;
+      apply reds
+    case _ h => cases h; case _ w h =>
+      apply Or.inr;
+      generalize tlp : List.map (· `@c η2) w = tl' at *; symm at tlp;
+      have reds : ∃ t', Red Γ (η1 `@c η2) t' := Exists.intro tl' (Red.appc_congr1 h tlp);
+      apply reds
+  case _ h => cases h; case _ w h =>
+    apply Or.inr;
+    generalize tlp : List.map (η1 `@c ·) w = tl' at *; symm at tlp;
+    have reds : ∃ t', Red Γ (η1 `@c η2) t' := Exists.intro tl' (Red.appc_congr2 h tlp);
+    apply reds
+
+case arrowc Γ A B η1 C D η2 _ _ η1J _ _ η2J _ _ η1s _ _ η2s =>
+  cases η2s (Judgment.wfempty wΓ) (DeclCtx.consempty ntype);
+  case _ h =>
+    have ntype' : DeclCtx (Frame.empty :: Γ) := DeclCtx.consempty ntype;
+    have η2refp := refl_is_val ntype' η2J h;
+    have η2refl := η2refp.1; cases (η1s wΓ ntype);
+    case _ h =>
+      have η1refp := refl_is_val ntype η1J h;
+      have η1refl := η1refp.1;
+      subst η1refl; subst η2refl;
+      apply Or.inr;
+      have reds : ∃ t', Red Γ (refl!(A) -c> refl! C) t' := Exists.intro [(refl! (A -t> C))] Red.arrowc;
+      apply reds
+    case _ h => cases h; case _ w h =>
+      apply Or.inr;
+      generalize tlp : List.map (· -c> η2) w = tl' at *; symm at tlp;
+      have reds : ∃ t', Red Γ (η1 -c> η2) t' := Exists.intro tl' (Red.arrowc_congr1 h tlp);
+      apply reds
+  case _ h => cases h; case _ w h =>
+    apply Or.inr;
+    generalize tlp : List.map (η1 -c> ·) w = tl' at *; symm at tlp;
+    have reds : ∃ t', Red Γ (η1 -c> η2) t' := Exists.intro tl' (Red.arrowc_congr2 h tlp);
+    apply reds
+
+case fst Γ A _ _ _ η C _ _ _ ηJ _ _ ηs =>
+  cases (ηs wΓ ntype);
+  case inl h =>
+    have ηrp := refl_is_val ntype ηJ h; have ηrfl := ηrp.1; subst ηrfl;
+    apply Or.inr;
+    have reds : ∃ t', Red Γ ((refl! (A `@k C)).!1) t' := Exists.intro [refl! A] Red.fst;
+    apply reds;
+  case inr h => cases h; case _ w h =>
+    apply Or.inr;
+    generalize tlp : List.map (·.!1) w = tl' at *; symm at tlp;
+    have reds : ∃ t', Red Γ (η.!1) t' := Exists.intro tl' (Red.fst_congr h tlp);
+    apply reds
+
+case snd Γ _ C _ η A _ _ _ _ ηJ _ _ _ ηs =>
+  cases (ηs wΓ ntype);
+  case inl h =>
+    have ηrp := refl_is_val ntype ηJ h; have ηrfl := ηrp.1; subst ηrfl;
+    apply Or.inr;
+    have reds : ∃ t', Red Γ ((refl! (A `@k C)).!2) t' := Exists.intro [refl! C] Red.snd;
+    apply reds;
+  case inr h => cases h; case _ w h =>
+    apply Or.inr;
+    generalize tlp : List.map (·.!2) w = tl' at *; symm at tlp;
+    have reds : ∃ t', Red Γ (η.!2) t' := Exists.intro tl' (Red.snd_congr h tlp);
+    apply reds
+
+case _ Γ K A B η allAJ allBJ ηJ _ _ ts =>
+  cases allAJ; case _ kkind _ =>
+  have ts := ts (Judgment.wfkind kkind wΓ) (DeclCtx.conskind ntype);
+  cases ts;
+  case inr h => cases h; case _ w h =>
+    simp_all;
+    apply Or.inr;
+    generalize tlp : List.map (∀c[K]·) w = tl' at *; symm at tlp;
+    have reds : ∃ t', Red Γ (∀c[K] η) t' := Exists.intro tl' (Red.allc_congr h tlp);
+    apply reds
+  case inl h =>
+    have ηrp := refl_is_val (DeclCtx.conskind ntype) ηJ h; have ηrfl := ηrp.1; subst ηrfl;
+    apply Or.inr;
+    have reds : ∃ t', Red Γ ((∀c[K] refl! A)) t' := Exists.intro [refl! (∀[K]A)] Red.allc;
+    apply reds;
+
+case _ Γ η1 K A B C D η2 _ _ η1J CKJ _ η2J _ _ η1s _ _ η2s =>
+  cases (η2s wΓ ntype);
+  case _ h =>
+    have η2refp := refl_is_val ntype η2J h;
+    have η2refl := η2refp.1; cases (η1s wΓ ntype);
+    case _ h =>
+      have η1refp := refl_is_val ntype η1J h;
+      have η1refl := η1refp.1;
+      subst η1refl; subst η2refl;
+      apply Or.inr;
+      have reds : ∃ t', Red Γ (refl!(∀[K] A) `@c[refl! C]) t' := Exists.intro [refl! (A β[ C ])] Red.apptc;
+      apply reds
+    case _ h => cases h; case _ w h =>
+      apply Or.inr;
+      generalize tlp : List.map (· `@c[η2]) w = tl' at *; symm at tlp;
+      have reds : ∃ t', Red Γ (η1 `@c[η2]) t' := Exists.intro tl' (Red.apptc_congr1 h tlp);
+      apply reds
+  case _ h => cases h; case _ w h =>
+    apply Or.inr;
+    generalize tlp : List.map (η1 `@c[·]) w = tl' at *; symm at tlp;
+    have reds : ∃ t', Red Γ (η1 `@c[η2]) t' := Exists.intro tl' (Red.apptc_congr2 h tlp);
+    apply reds
